@prefix : <https://rs.tdwg.org/bdqffdq/terms#> .
@prefix owl: <http://www.w3.org/2002/07/owl#> .
@prefix rdf: <http://www.w3.org/1999/02/22-rdf-syntax-ns#> .
@prefix xml: <http://www.w3.org/XML/1998/namespace> .
@prefix xsd: <http://www.w3.org/2001/XMLSchema#> .
@prefix rdfs: <http://www.w3.org/2000/01/rdf-schema#> .
@prefix skos: <http://www.w3.org/2004/02/skos/core#> .
@prefix bdqffdq: <https://rs.tdwg.org/bdqffdq/terms/> .
@prefix dcterms: <http://purl.org/dc/terms/> .
@base <https://rs.tdwg.org/bdqffdq/terms> .

<https://rs.tdwg.org/bdqffdq/terms> rdf:type owl:Ontology ;
                                     rdfs:comment "The classes and object properties found in this ontology are dedicated to fundamental and derived concepts from the Fitness For Use Framework described in the paper by Veiga et al available at: http://journals.plos.org/plosone/article?id=10.1371/journal.pone.0178731 as modified to describe data quality fitness for use tests in the BDQ Core (draft) TDWG Standard." ;
                                     rdfs:label "Biodiversity Data Quality Fitness for Use Framework" .

#################################################################
#    Annotation properties
#################################################################

###  http://purl.org/dc/terms/issued
dcterms:issued rdf:type owl:AnnotationProperty .


###  http://www.w3.org/1999/02/22-rdf-syntax-ns#value
rdf:value rdf:type owl:AnnotationProperty .


###  http://www.w3.org/2004/02/skos/core#definition
skos:definition rdf:type owl:AnnotationProperty .


###  http://www.w3.org/2004/02/skos/core#prefLabel
skos:prefLabel rdf:type owl:AnnotationProperty .


#################################################################
#    Datatypes
#################################################################

###  http://www.w3.org/2001/XMLSchema#date
xsd:date rdf:type rdfs:Datatype .


#################################################################
#    Object Properties
#################################################################

###  https://rs.tdwg.org/bdqffdq/terms/amendmentProperty
bdqffdq:amendmentProperty rdf:type owl:ObjectProperty ;
                          dcterms:issued "2024-09-30"^^xsd:date ;
                          rdfs:comment "Sub properties of this type group object properties that apply to amendment concepts such as AmendmentPolicy (DQ Needs), AmendmentMethod (DQ Solutions) and Amendment (DQ Reports)." ;
                          rdfs:label "amendment Property" ;
                          skos:definition "Category of object properties that apply to Amendmentts" ;
                          skos:prefLabel "amendment Property" .


###  https://rs.tdwg.org/bdqffdq/terms/appliesTo
bdqffdq:appliesTo rdf:type owl:ObjectProperty ;
                  dcterms:issued "2024-09-30"^^xsd:date ;
                  rdfs:comment "If an Assertion forms the oa:body of an oa:Annotation, the appliesTo DataResource would be the oa:target of the Annotation.  If Assertions are composed in DataQualityReports, the appliesTo DataResource is an item examined as part of the report.  Expectation for SingleRecord test Assertions on Darwin Core data in BDQ Core is that appliesTo would point at an Occurrence." ;
                  rdfs:label "applies To" ;
                  skos:definition "Describes the DataResource about which an Assertion is made." ;
                  skos:prefLabel "applies To" .


###  https://rs.tdwg.org/bdqffdq/terms/composedOf
bdqffdq:composedOf rdf:type owl:ObjectProperty ;
                   dcterms:issued "2024-09-30"^^xsd:date ;
                   rdfs:comment "Describes the properties from a controlled vocabulary that compose an InformationElement. For example, an InformationElement may be composedOf properties such as dwc:day, dwc:month and dwc:year." ;
                   rdfs:label "composed Of" ;
                   skos:definition "Specific vocabulary term that comprises a non-abstract InformationElement." ;
                   skos:prefLabel "composed Of" .


###  https://rs.tdwg.org/bdqffdq/terms/containsAssertion
bdqffdq:containsAssertion rdf:type owl:ObjectProperty ;
                          dcterms:issued "2024-09-30"^^xsd:date ;
                          rdfs:comment "Connects Assertions together into Data Quality Reports.  Alterntatively, Assertions can be contained in oa:Annotations, in which case this property is not used." ;
                          rdfs:label "contains Assertion" ;
                          skos:definition "Connects a Data Quality Report with Assertions that comprise that report." ;
                          skos:prefLabel "contains Assertion" .


###  https://rs.tdwg.org/bdqffdq/terms/forAmendment
bdqffdq:forAmendment rdf:type owl:ObjectProperty ;
                     rdfs:subPropertyOf bdqffdq:amendmentProperty ,
                                        bdqffdq:forDataQualityNeed ;
                     rdfs:range [ rdf:type owl:Restriction ;
                                  owl:onProperty bdqffdq:forAmendment ;
                                  owl:someValuesFrom bdqffdq:Amendment
                                ] ;
                     dcterms:issued "2024-09-30"^^xsd:date ;
                     rdfs:comment "Use to link AmendmentMethods to Amendments.  Describes the relationship between an AmendmentMethod (solutions) and an Amendment (needs)." ;
                     rdfs:label "for Amendment" ;
                     skos:definition "Relates an AmendmentMethod to an Amendment." ;
                     skos:prefLabel "for Amendment" .


###  https://rs.tdwg.org/bdqffdq/terms/forDataQualityNeed
bdqffdq:forDataQualityNeed rdf:type owl:ObjectProperty ;
                           dcterms:issued "2024-09-30"^^xsd:date ;
                           rdfs:comment "Category of properties that link tests to their Methods." ;
                           rdfs:label "for Data Quality Need" ;
                           skos:definition "Category of properties that relates specific Data Quality Needs to specific Methods." ;
                           skos:prefLabel "for Data Quality Need" .


###  https://rs.tdwg.org/bdqffdq/terms/forIssue
bdqffdq:forIssue rdf:type owl:ObjectProperty ;
                 rdfs:subPropertyOf bdqffdq:forDataQualityNeed ,
                                    bdqffdq:issueProperty ;
                 rdfs:range [ rdf:type owl:Restriction ;
                              owl:onProperty bdqffdq:forIssue ;
                              owl:someValuesFrom bdqffdq:Issue
                            ] ;
                 dcterms:issued "2024-09-30"^^xsd:date ;
                 rdfs:comment "Use to link IssueMethods to Issues.  Describes the relationship between a IssueMethod (solutions) in bdqffdq and an Issue (needs).  Paralell concepts are forAmendment, forValidation, forMeasure." ;
                 rdfs:label "for Issue" ;
                 skos:definition "Relates an IssuetMethod to an Issue." ;
                 skos:prefLabel "for Issue" .


###  https://rs.tdwg.org/bdqffdq/terms/forMeasure
bdqffdq:forMeasure rdf:type owl:ObjectProperty ;
                   rdfs:subPropertyOf bdqffdq:forDataQualityNeed ,
                                      bdqffdq:measurementProperty ;
                   rdfs:range [ rdf:type owl:Restriction ;
                                owl:onProperty bdqffdq:forMeasure ;
                                owl:someValuesFrom bdqffdq:Measure
                              ] ;
                   dcterms:issued "2024-09-30"^^xsd:date ;
                   rdfs:comment "Use to link MeasurementMethods (solutions) to Measures (needs).   Paralell concepts are forAmendment, forValidation, forIssue." ;
                   rdfs:label "for Measure" ;
                   skos:definition "Relates an MeasurementMethod to a Measure." ;
                   skos:prefLabel "for Measure" .


###  https://rs.tdwg.org/bdqffdq/terms/forValidation
bdqffdq:forValidation rdf:type owl:ObjectProperty ;
                      rdfs:subPropertyOf bdqffdq:forDataQualityNeed ,
                                         bdqffdq:validationProperty ;
                      rdfs:range [ rdf:type owl:Restriction ;
                                   owl:onProperty bdqffdq:forValidation ;
                                   owl:someValuesFrom bdqffdq:Validation
                                 ] ;
                      dcterms:issued "2024-09-30"^^xsd:date ;
                      rdfs:comment "Use to link ValidationMethods to Validations.  Describes the relationship between a ValidationMethod (solutions) and a Validation (needs).   Paralell concepts are forAmendment, forMeasure, and forIssue."@en ;
                      rdfs:label "for Validation"@en ;
                      skos:definition "Relates an ValidationMethod to a Validation." ;
                      skos:prefLabel "for Validation"@en .


###  https://rs.tdwg.org/bdqffdq/terms/hasActedUponInformationElement
bdqffdq:hasActedUponInformationElement rdf:type owl:ObjectProperty ;
                                       rdfs:subPropertyOf bdqffdq:hasInformationElement ;
                                       dcterms:issued "2024-09-30"^^xsd:date ;
                                       rdfs:comment "Provides a relationship between bdqffdq concepts and the information elements that are ActedUpon in a test."@en ;
                                       rdfs:label "has Acted Upon Information Element" ;
                                       skos:definition "Describes the ActedUpon InformationElements assessed by a DataQualityNeed about which Assertions arising from the DataQualityNeed would apply." ;
                                       skos:prefLabel "has Acted Upon Information Element" .


###  https://rs.tdwg.org/bdqffdq/terms/hasArgument
bdqffdq:hasArgument rdf:type owl:ObjectProperty ;
                    rdfs:range bdqffdq:Argument ;
                    dcterms:issued "2024-09-30"^^xsd:date ;
                    rdfs:comment "Expected to be a relationship between a Specification and an Argument, where the Argument provides a value for a Paramter (e.g. bdq:sourceAuthority), and a hasAuthoritiesDefaults for the Specification may provide a default value for the Parameter under that specification." ;
                    rdfs:label "has Argument" ;
                    skos:definition "Relates a Specification to an Argument" ;
                    skos:prefLabel "has Argument" .


###  https://rs.tdwg.org/bdqffdq/terms/hasConsultedInformationElement
bdqffdq:hasConsultedInformationElement rdf:type owl:ObjectProperty ;
                                       rdfs:subPropertyOf bdqffdq:hasInformationElement ;
                                       dcterms:issued "2024-09-30"^^xsd:date ;
                                       rdfs:comment "Provides a relationship between bdqffdq concepts and the information elements that are Consulted, but not ActedUpon in a test."@en ;
                                       rdfs:label "has Consulted Information Element" ;
                                       skos:definition "Describes the InformationElements assessed by a DataQualityNeed in order to make Assertions concerning ActedUpon InformationElements." ;
                                       skos:prefLabel "has Consulted Information Element" .


###  https://rs.tdwg.org/bdqffdq/terms/hasCriterion
bdqffdq:hasCriterion rdf:type owl:ObjectProperty ;
                     rdfs:subPropertyOf bdqffdq:issueProperty ,
                                        bdqffdq:validationProperty ;
                     rdfs:range [ rdf:type owl:Restriction ;
                                  owl:onProperty bdqffdq:hasCriterion ;
                                  owl:someValuesFrom bdqffdq:Criterion
                                ] ;
                     dcterms:issued "2024-09-30"^^xsd:date ;
                     rdfs:comment "Used to link the derived concept of a Validation to the fundamental concept of a Criterion."@en ;
                     rdfs:label "has Criterion"@en ;
                     skos:definition "The Criterion under which a Validation or Issue assesses for data quality." ;
                     skos:prefLabel "has Criterion"@en .


###  https://rs.tdwg.org/bdqffdq/terms/hasDataQualityDimension
bdqffdq:hasDataQualityDimension rdf:type owl:ObjectProperty ;
                                rdfs:subPropertyOf bdqffdq:amendmentProperty ,
                                                   bdqffdq:issueProperty ,
                                                   bdqffdq:measurementProperty ,
                                                   bdqffdq:validationProperty ;
                                rdfs:range [ rdf:type owl:Restriction ;
                                             owl:onProperty bdqffdq:hasDataQualityDimension ;
                                             owl:someValuesFrom bdqffdq:DataQualityDimension
                                           ] ;
                                dcterms:issued "2024-09-30"^^xsd:date ;
                                rdfs:comment """Used to link a derived concept of a DataQualityNeed (a test, that is a Measure, Validation, Amendment, or Issue) to the fundamental concept of a DataQualityDimension.  For a Measure, the dimension of data quality measured.   For a Validation or Issue, the dimension of data quality assessed.  For an Amendment, the dimension of data quality to be improved.  

Under the original formulation of the Framework, only Measures have Dimensions.""" ;
                                rdfs:label "has Data Quality Dimension"@en ;
                                skos:definition "The DataQualityDimension to which a DataQualityNeed Applies." ;
                                skos:prefLabel "has Data Quality Dimension"@en .


###  https://rs.tdwg.org/bdqffdq/terms/hasEnhancement
bdqffdq:hasEnhancement rdf:type owl:ObjectProperty ;
                       rdfs:subPropertyOf bdqffdq:amendmentProperty ;
                       rdfs:range [ rdf:type owl:Restriction ;
                                    owl:onProperty bdqffdq:hasEnhancement ;
                                    owl:someValuesFrom bdqffdq:Enhancement
                                  ] ;
                       dcterms:issued "2024-09-30"^^xsd:date ;
                       rdfs:comment "Used to link the derived property of an Amendment to the Fundamental property of an Enhancement." ;
                       rdfs:label "has Enhancement" ;
                       skos:definition "The Enhancement that describes how an Amendment may propose changes to improve data quality." ;
                       skos:prefLabel "has Enhancement" .


###  https://rs.tdwg.org/bdqffdq/terms/hasInformationElement
bdqffdq:hasInformationElement rdf:type owl:ObjectProperty ;
                              rdfs:subPropertyOf bdqffdq:amendmentProperty ,
                                                 bdqffdq:issueProperty ,
                                                 bdqffdq:measurementProperty ,
                                                 bdqffdq:validationProperty ;
                              rdfs:range bdqffdq:InformationElement ;
                              dcterms:issued "2024-09-30"^^xsd:date ;
                              rdfs:comment """Provides a relationship between DataQualityNeeds concepts and Information elements. For example, Validation uses this property along with hasResourceType to define a criterion in the context of related information elements.

Subtypes hasActedUponInformationElement and hasConsultedInformationElement allow data quality needs to be related to specific information element terms in a way that allows data quality reports to distinguish for consumers which information elements a test makes assertions about (and which only informed that assertion).""" ;
                              rdfs:label "has Information Element" ;
                              skos:definition "Describes the InformationElements assessed by a DataQualityNeed." ;
                              skos:prefLabel "has Information Element" .


###  https://rs.tdwg.org/bdqffdq/terms/hasParameter
bdqffdq:hasParameter rdf:type owl:ObjectProperty ;
                     rdfs:range bdqffdq:Parameter ;
                     dcterms:issued "2024-09-30"^^xsd:date ;
                     rdfs:comment "Expected to be a relationship between a Specification and a Parameter, where the Parameter defines the term for the parameter (e.g. bdq:sourceAuthority), and a hasAuthoritiesDefaults for the Specification provides a default value for the Parameter under that specification."@en ;
                     rdfs:label "has Parameter"@en ;
                     skos:definition "Relates an Argument to a Parameter."@en ;
                     skos:prefLabel "has Parameter"@en .


###  https://rs.tdwg.org/bdqffdq/terms/hasResourceType
bdqffdq:hasResourceType rdf:type owl:ObjectProperty ;
                        dcterms:issued "2024-09-30"^^xsd:date ;
                        rdfs:comment "Provides additional metadata, along with the information elements, that describe the nature of the data  (SingleRecord or MultiRecord) on which the bdqffdq concept operates. For example, an Amendment with resource type of MultiRecord defines that Amendment as operating on a data set." ;
                        rdfs:label "has Resource Type" ;
                        skos:definition "Resource Type to which a DataQualityNeed applies." ;
                        skos:prefLabel "has Resource Type" .


###  https://rs.tdwg.org/bdqffdq/terms/hasResponseQualifier
bdqffdq:hasResponseQualifier rdf:type owl:ObjectProperty ;
                             rdfs:subPropertyOf bdqffdq:reportProperty ;
                             dcterms:issued "2024-09-30"^^xsd:date ;
                             rdfs:comment "Optional extension point, could be used to add structured information about uncertainty."@en ;
                             rdfs:label "has Response Qualifier"@en ;
                             skos:definition "ResponseQualifier object asserted by an Assertion." ;
                             skos:prefLabel "has Response Qualifier"@en .


###  https://rs.tdwg.org/bdqffdq/terms/hasResponseResult
bdqffdq:hasResponseResult rdf:type owl:ObjectProperty ;
                          rdfs:subPropertyOf bdqffdq:reportProperty ;
                          dcterms:issued "2024-09-30"^^xsd:date ;
                          rdfs:comment """Used in the DQ Report concept to describe response result objects. For example, values could be bdqffdq:COMPLIANT or bdqffdq:NOT_COMPLIANT for ValidationAssertions.   ValidationAssertions and IssueAssertions have ResponseResults as objects.  AmendmentAssertions have ResponseResults that are data properties, so they are not expected to use this object property.  MeasurementAssertion ResponseResults may be objects or data.  

 If Response.results are not objects, use the datatype property hasResponseResultValue"""@en ;
                          rdfs:label "has Response Result" ;
                          skos:definition "ResponseResult object asserted by an Assertion." ;
                          skos:prefLabel "has Response Result" .


###  https://rs.tdwg.org/bdqffdq/terms/hasResponseStatus
bdqffdq:hasResponseStatus rdf:type owl:ObjectProperty ;
                          rdfs:subPropertyOf bdqffdq:reportProperty ;
                          dcterms:issued "2024-09-30"^^xsd:date ;
                          rdfs:comment """Used in the DQ Report concept to describe response status.  For example, in the case of a ValidationAssertion ResponseStatus values could be bdqffdq:RUN_HAS_RESULT or bdqffdq:INTERNAL_PREREQUISITES_NOT_MET, or bdqffdq:EXTERNAL_PREREQISITES_NOT_MET.   Similarly, AmendmentAssertions can assert ResponesStatus objects including bdqffdq:AMENDED or bdqffdq:FILLED_IN.  

ResponseStatus is always an object, unlike ResponseResult, where either the object property hasResponseResult or the data property hasResponseResultValue may apply.""" ;
                          rdfs:label "has Response Status" ;
                          skos:definition "ResponseStatus object asserted by an Assertion." ;
                          skos:prefLabel "has Response Status" .


###  https://rs.tdwg.org/bdqffdq/terms/hasSpecification
bdqffdq:hasSpecification rdf:type owl:ObjectProperty ;
                         rdfs:range [ rdf:type owl:Restriction ;
                                      owl:onProperty bdqffdq:hasSpecification ;
                                      owl:someValuesFrom bdqffdq:Specification
                                    ] ;
                         dcterms:issued "2024-09-30"^^xsd:date ;
                         rdfs:comment "Describes the relationship between a derived bdqffdq concept that is a Method and the fundamental concept of a Specification (technical description of a test)." ;
                         rdfs:label "has Specification" ;
                         skos:definition "Relates a Method to a Specification." ;
                         skos:prefLabel "has Specification" .


###  https://rs.tdwg.org/bdqffdq/terms/hasUseCase
bdqffdq:hasUseCase rdf:type owl:ObjectProperty ;
                   rdfs:range [ rdf:type owl:Restriction ;
                                owl:onProperty bdqffdq:hasUseCase ;
                                owl:someValuesFrom bdqffdq:UseCase
                              ] ;
                   dcterms:issued "2024-09-30"^^xsd:date ;
                   rdfs:comment "Used by concepts in the DQ Needs category to describe the relationship between DQ Policies (ValidationPolicy, AmendmentPolicy, MeasurementPolicy) and an instance of a UseCase." ;
                   rdfs:label "has Use Case" ;
                   skos:definition "Relates a Policy to a UseCase." ;
                   skos:prefLabel "has Use Case" .


###  https://rs.tdwg.org/bdqffdq/terms/implementedBy
bdqffdq:implementedBy rdf:type owl:ObjectProperty ;
                      rdfs:range [ rdf:type owl:Restriction ;
                                   owl:onProperty bdqffdq:implementedBy ;
                                   owl:someValuesFrom bdqffdq:Mechanism
                                 ] ;
                      dcterms:issued "2024-09-30"^^xsd:date ;
                      rdfs:comment "Describes the link between the Implementation concept in bdqffdq and a Mechanism." ;
                      rdfs:label "implemented By" ;
                      skos:definition "Mechanism that provides an Implementation" ;
                      skos:prefLabel "implemented By" .


###  https://rs.tdwg.org/bdqffdq/terms/improvedBy
bdqffdq:improvedBy rdf:type owl:ObjectProperty ;
                   rdfs:range [ rdf:type owl:Restriction ;
                                owl:onProperty bdqffdq:improvedBy ;
                                owl:someValuesFrom bdqffdq:Amendment
                              ] ;
                   dcterms:issued "2024-09-30"^^xsd:date ;
                   rdfs:comment """Origially had Domain: Amendment and Range: ImprovementTarget.   Asserts that an improvement target could be improved by the Amendment.  

Object property that describes an Amenement, as part of the ImprovementTarget, that would improve data acted upon by some set of Measures or Validations.  This can be used to determine which Measures and Validations are improved upon by a given Amendment.""" ;
                   rdfs:label "improved By" ;
                   skos:definition "ImprovementTarget that would have data quality improved by assertions resulting from an Amendment." ;
                   skos:prefLabel "improved By" .


###  https://rs.tdwg.org/bdqffdq/terms/includedInPolicy
bdqffdq:includedInPolicy rdf:type owl:ObjectProperty ;
                         dcterms:issued "2024-09-30"^^xsd:date ;
                         rdfs:comment "Relates Policies to tests (DataQualityNeeds) ." ;
                         rdfs:label "included in Policy" ;
                         skos:definition "Assserts that a Data Quality Need is part of a Policy" ;
                         skos:prefLabel "included In Policy" .


###  https://rs.tdwg.org/bdqffdq/terms/issueProperty
bdqffdq:issueProperty rdf:type owl:ObjectProperty ;
                      dcterms:issued "2024-09-30"^^xsd:date ;
                      rdfs:comment "Properties that relate Issues to IssueMethods, Criteria, and dataQualityDimensions." ;
                      rdfs:label "issue Property" ;
                      skos:definition "Category of object properties that apply to Issues." ;
                      skos:prefLabel "issue Property" .


###  https://rs.tdwg.org/bdqffdq/terms/measurementProperty
bdqffdq:measurementProperty rdf:type owl:ObjectProperty ;
                            dcterms:issued "2024-09-30"^^xsd:date ;
                            rdfs:comment "Sub properties of this type group object properties that apply to measurement concepts such as MeasurementPolicy (DQ Needs), MeasurementMethod (DQ Solutions) and Measure (DQ Reports)." ;
                            rdfs:label "measurement Property" ;
                            skos:definition "Category of object properties that apply to Measures." ;
                            skos:prefLabel "measurement Property" .


###  https://rs.tdwg.org/bdqffdq/terms/producesAssertion
bdqffdq:producesAssertion rdf:type owl:ObjectProperty ;
                          dcterms:issued "2024-09-30"^^xsd:date ;
                          rdfs:comment "Connects Implementations (solutions) with the Assertions (reports) that they produce from the execution of a Specification." ;
                          rdfs:label "produces Assertion" ;
                          skos:definition "Connects an entity with an assertion that the entity created." ;
                          skos:prefLabel "produces Assertion" .


###  https://rs.tdwg.org/bdqffdq/terms/reportProperty
bdqffdq:reportProperty rdf:type owl:ObjectProperty ;
                       dcterms:issued "2024-09-30"^^xsd:date ;
                       rdfs:comment "Category of properties used in reports (object properties associated with Response objects (bdqffdq:Assertions)).  See also the data properties bdqffdq:hasResponseComment and bdqffdq:hasResponseResultValue." ;
                       rdfs:label "report Property" ;
                       skos:definition "Category of object properties that apply to Assertions." ;
                       skos:prefLabel "report Property" .


###  https://rs.tdwg.org/bdqffdq/terms/targetedIssue
bdqffdq:targetedIssue rdf:type owl:ObjectProperty ;
                      rdfs:range [ rdf:type owl:Restriction ;
                                   owl:onProperty bdqffdq:targetedIssue ;
                                   owl:someValuesFrom bdqffdq:Issue
                                 ] ;
                      dcterms:issued "2024-09-30"^^xsd:date ;
                      rdfs:comment "The issue targeted by some problem via the ImprovementTarget object.  Describes the relationship between an improvement target and an Issue." ;
                      rdfs:label "targeted Issue" ;
                      skos:definition "Issue where the data conformance with needs may be improved by accepting proposals from an Amendment via an ImprovementTarget." ;
                      skos:prefLabel "targeted Issue" .


###  https://rs.tdwg.org/bdqffdq/terms/targetedMeasure
bdqffdq:targetedMeasure rdf:type owl:ObjectProperty ;
                        rdfs:range [ rdf:type owl:Restriction ;
                                     owl:onProperty bdqffdq:targetedMeasure ;
                                     owl:someValuesFrom bdqffdq:Measure
                                   ] ;
                        dcterms:issued "2024-09-30"^^xsd:date ;
                        rdfs:comment "Describes the relationship between an improvement target and a Measure."@en ;
                        rdfs:label "targeted Measure"@en ;
                        skos:definition "Measure where the data conformance with needs may be improved by accepting proposals from an Amendment via an ImprovementTarget."@en ;
                        skos:prefLabel "targeted Measure"@en .


###  https://rs.tdwg.org/bdqffdq/terms/targetedValidation
bdqffdq:targetedValidation rdf:type owl:ObjectProperty ;
                           rdfs:subPropertyOf owl:topObjectProperty ;
                           rdfs:range [ rdf:type owl:Restriction ;
                                        owl:onProperty bdqffdq:targetedValidation ;
                                        owl:someValuesFrom bdqffdq:Validation
                                      ] ;
                           dcterms:issued "2024-09-30"^^xsd:date ;
                           rdfs:comment "Relates an improvement target to a Validation.  Describes the relationship between an improvement target and a Validation."@en ;
                           rdfs:label "targeted Validation"@en ;
                           skos:definition "Validation where the data conformance with needs may be improved by accepting proposals from an Amendment via an ImprovementTarget."@en ;
                           skos:prefLabel "targeted Validation"@en .


###  https://rs.tdwg.org/bdqffdq/terms/usesSpecification
bdqffdq:usesSpecification rdf:type owl:ObjectProperty ;
                          rdfs:range [ rdf:type owl:Restriction ;
                                       owl:onProperty bdqffdq:usesSpecification ;
                                       owl:someValuesFrom bdqffdq:Specification
                                     ] ;
                          dcterms:issued "2024-09-30"^^xsd:date ;
                          rdfs:comment "Relates an Implementation to the Specification that the Implementation implements." ;
                          rdfs:label "uses Specification" ;
                          skos:definition "Specification that an Implementation implements." ;
                          skos:prefLabel "uses Specification" .


###  https://rs.tdwg.org/bdqffdq/terms/validationProperty
bdqffdq:validationProperty rdf:type owl:ObjectProperty ;
                           dcterms:issued "2024-09-30"^^xsd:date ;
                           rdfs:comment "Sub properties of this type group object properties that apply to validation concepts such as ValidationPolicy (DQ Needs), ValidationMethod (DQ Solutions) and Validation (DQ Reports)." ;
                           rdfs:label "validation Property" ;
                           skos:definition "Category of object properties that apply to Validations." ;
                           skos:prefLabel "validation Property" .


#################################################################
#    Data properties
#################################################################

###  https://rs.tdwg.org/bdqffdq/terms/hasArgumentValue
bdqffdq:hasArgumentValue rdf:type owl:DatatypeProperty ;
                         dcterms:issued "2024-09-30"^^xsd:date ;
                         rdfs:label "has Argument value" ;
                         skos:definition "The value of an Argument which is used in a Specification to replace a formal Parameter to determine the behavior of the Specification." ;
                         skos:prefLabel "has Argument value" .


###  https://rs.tdwg.org/bdqffdq/terms/hasAuthoritiesDefaults
bdqffdq:hasAuthoritiesDefaults rdf:type owl:DatatypeProperty ;
                               rdfs:range xsd:string ;
                               dcterms:issued "2024-09-30"^^xsd:date ;
                               rdfs:comment "Details of the bdq:sourceAuthority listed in a Specification, along with Parameters that may be provided to the expected response along with their default values." ;
                               rdfs:label "has Authorities and Defaults"@en ;
                               skos:definition "Text describing source authorities and parameters with their default values to attach to a Specification to further specify the behavior described in the expected response." ;
                               skos:prefLabel "has Authorities and Defaults" .


###  https://rs.tdwg.org/bdqffdq/terms/hasDateLastUpdated
bdqffdq:hasDateLastUpdated rdf:type owl:DatatypeProperty ;
                           rdfs:subPropertyOf owl:topDataProperty ;
                           rdfs:range xsd:date ;
                           dcterms:issued "2024-09-30"^^xsd:date ;
                           rdfs:comment "While a new instance of a resource with a new dcterms:issued is required for any change to that resource, not all changes would be pertenent to implemeters, that is would required implementers to evaluate their code for changes needed to comply with the update.  bdqffdq:hasDateLastUpdated allows implementers to identify which new changes to the definition of a test would entail changes to code, and which would not.   For example, a change to the logic of a Specification in the text of hasExpectedResponse would imply needed changes to the logic of code implementing that specification, but a correction of a spelling mistake within the text of a hasExpectedResponse would not." ;
                           rdfs:label "has Date Last Updated" ;
                           skos:definition "Date of the most recent dcterms:Issued for this class with a change that would be pertenent to implementation." ;
                           skos:prefLabel "has Date Last Updated" .


###  https://rs.tdwg.org/bdqffdq/terms/hasExpectedResponse
bdqffdq:hasExpectedResponse rdf:type owl:DatatypeProperty ;
                            rdfs:range xsd:string ;
                            dcterms:issued "2024-09-30"^^xsd:date ;
                            rdfs:comment "The description of the logic of a test Specification.  An expected response is expected to be a data property of a Specification."@en ;
                            rdfs:label "has Expected Response"@en ;
                            skos:definition "Text describing the logic to be followed by an implementation of a Specification specifying the values of ResponseStatus and ResponseResults that should be produced from the evaluation of input InformationElements." ;
                            skos:prefLabel "has Expected Response"@en .


###  https://rs.tdwg.org/bdqffdq/terms/hasResponseComment
bdqffdq:hasResponseComment rdf:type owl:DatatypeProperty ;
                           rdfs:range xsd:string ;
                           dcterms:issued "2024-09-30"^^xsd:date ;
                           rdfs:comment "Intended for consumption by human readers of data quality reports to understand why particular assertions were made.  Referenced in some documentation as Response.comment." ;
                           rdfs:label "has Response Comment" ;
                           skos:definition "Free text describing the assertion made in the response and why that conclusion was reached." ;
                           skos:prefLabel "has Response Comment" .


###  https://rs.tdwg.org/bdqffdq/terms/hasResponseResultValue
bdqffdq:hasResponseResultValue rdf:type owl:DatatypeProperty ;
                               dcterms:issued "2024-09-30"^^xsd:date ;
                               rdfs:comment "Applies to AmendmentAssertions.   To support bdqcore: tests, is expected to carry a key:value list where the keys are the names of ActedUpon InformationElements, and the values are the proposed new values (filling in or replacing the values of those terms in the input).  Applies to MeasureAssertions that assert a numeric value." ;
                               rdfs:label "has response result value" ;
                               skos:definition "Data property carrying the value of an Assertion when not an object." ;
                               skos:prefLabel "has response result value" .


#################################################################
#    Classes
#################################################################

###  https://rs.tdwg.org/bdqffdq/terms/AbstractInformationElement
bdqffdq:AbstractInformationElement rdf:type owl:Class ;
                                   rdfs:subClassOf bdqffdq:InformationElement ;
                                   dcterms:issued "2024-09-30"^^xsd:date ;
                                   rdfs:comment "Information elements such as DATE and DAY are abstract, they could reference any representation of those concepts.  In contrast, dwc:eventDate and dwc:day can be linked to concrete Acted Upon or Consulted information elements." ;
                                   rdfs:label "Abstract Information Element" ;
                                   skos:definition "An InformationElement described in abstract terms and not linked with one or more concrete terms." ;
                                   skos:prefLabel "Abstract Information Element" .


###  https://rs.tdwg.org/bdqffdq/terms/ActedUpon
bdqffdq:ActedUpon rdf:type owl:Class ;
                  rdfs:subClassOf bdqffdq:InformationElement ;
                  dcterms:issued "2024-09-30"^^xsd:date ;
                  rdfs:comment "An information element to which a Result applies."@en ;
                  rdfs:label "Acted Upon"@en ;
                  skos:definition "An information element, expressed in concrete terms, about which a data quality need expresses assertions about the data quality in that element." ;
                  skos:prefLabel "Acted Upon" .


###  https://rs.tdwg.org/bdqffdq/terms/Amendment
bdqffdq:Amendment rdf:type owl:Class ;
                  rdfs:subClassOf bdqffdq:AmendmentConcept ,
                                  bdqffdq:DataQualityNeed ;
                  dcterms:issued "2024-09-30"^^xsd:date ;
                  rdfs:comment """ContextualizedEnhacement in the original framework.   Describes an instance of the enhancement concept in the context of the associated information elements from some controlled vocabulary (fields ActedUpon or Consulted), and a ResourceType of SingleRecord or MultiRecord.  

Describes a proposal for enhancement of original data, which if accepted, would improve the quality of the data for some use. For example: Recommends valid value for taxon name in a single record.  

Amendments may describe proposed changes to data values, or proposed changes to processes for the production and manipulation of data, for example an Amendment on a SingleRecord may provide criteria for proposing that latitude and longitude are transposed in that record, or a similar Amendment on a MultiRecord may provide critera for proposing that all latitudes and longitudes from some data source have been transposed, and the mapping of data values to transport terms should be changed.  

An Amendment is the data quality needs concept that parallels an AmendmentMethod at the solutions level, and an AmendmentAssertion at the report level.   

AM = { am | am = < ie, e, rt >, ie ∈ IE, e ∈ E ⋀ rt ∈ RT }"""@en ;
                  rdfs:label "Amendment"@en ;
                  skos:definition "A data quality need that expresses how proposals may be made to improve the fitness for use of data." ;
                  skos:prefLabel "Amendment"@en .


###  https://rs.tdwg.org/bdqffdq/terms/AmendmentAssertion
bdqffdq:AmendmentAssertion rdf:type owl:Class ;
                           rdfs:subClassOf bdqffdq:AmendmentConcept ,
                                           bdqffdq:Assertion ;
                           dcterms:issued "2024-09-30"^^xsd:date ;
                           rdfs:comment """The Amendment assertion type is a report level concept that describes the results of the execution of of a test that performs an AmendmentMethod following some Specification to propose changes based on some Amendment. 

An Amendment concept in bdqffdq is expected to carry a ResponseStatus result that includes a status FILLED_IN, AMENDED, as well as a ResponseResult that asserts proposed changes to values from the original data.

DQA(dr) = {dqa | dqa = < am, s, m, r >, am ∈ AM, s ∈ S, m ∈ M , r ∈ R ⋀ dr ∈ DR}""" ;
                           rdfs:label "Amendment Assertion"@en ;
                           skos:definition "An assertion expressing the result of an implementation evaluating an amendment supporting a particular data quality need to improve a particular data resource." ;
                           skos:prefLabel "Amendment Assertion"@en .


###  https://rs.tdwg.org/bdqffdq/terms/AmendmentConcept
bdqffdq:AmendmentConcept rdf:type owl:Class ;
                         dcterms:issued "2024-09-30"^^xsd:date ;
                         rdfs:label "Amendment Concept"@en ;
                         skos:definition "A term involved in proposals of changes to data or process to improve data quallity to fit expressed data quality needs."@en ;
                         skos:prefLabel "Amendment Concept"@en .


###  https://rs.tdwg.org/bdqffdq/terms/AmendmentMethod
bdqffdq:AmendmentMethod rdf:type owl:Class ;
                        rdfs:subClassOf bdqffdq:AmendmentConcept ,
                                        bdqffdq:DataQualityMethod ;
                        dcterms:issued "2024-09-30"^^xsd:date ;
                        rdfs:comment """The AmendmentMethod in bdqffdq is a DQ Solutions level concept describing the relationship between a Specification (technical description of a test) and an Amendment (an enhancement in the context of resource type (SingleRecord or MultiRecord) and associated information elements).

EM(am) = {s | s ⊂ S ⋀ am ∈ AM}""" ;
                        rdfs:label "Amendment Method"@en ;
                        skos:definition "A data quality solution concept that relates an Amendment to its Specifications." ;
                        skos:prefLabel "Amendment Method"@en .


###  https://rs.tdwg.org/bdqffdq/terms/AmendmentPolicy
bdqffdq:AmendmentPolicy rdf:type owl:Class ;
                        rdfs:subClassOf bdqffdq:AmendmentConcept ,
                                        bdqffdq:Policy ;
                        dcterms:issued "2024-09-30"^^xsd:date ;
                        rdfs:comment """A Data Quality needs level concept that describes how some Amendment relates to a UseCase. This relationship defines which amendments are supported by a given UseCase.

EP(u) = {am | am ⊂ AM ⋀ u ∈ U }""" ;
                        rdfs:label "Amendment Policy"@en ;
                        skos:definition "A need concept that relates a UseCase to a set of supporting Amendments."@en ;
                        skos:prefLabel "Amendment Policy"@en .


###  https://rs.tdwg.org/bdqffdq/terms/Argument
bdqffdq:Argument rdf:type owl:Class ;
                 rdfs:subClassOf bdqffdq:SolutionsConcept ;
                 dcterms:issued "2024-09-30"^^xsd:date ;
                 rdfs:comment "The argument is an Actual Parameter, for which a Parameter is the corresponding Formal Parameter.  An extension to the original fitness for use framework as described in Veiga et al., 2017."@en ;
                 rdfs:label "Argument" ;
                 skos:definition "A value that, when provided to a test Specification to replace a Parameter changes the behavior of the test in a defined manner." ;
                 skos:prefLabel "Argument"@en .


###  https://rs.tdwg.org/bdqffdq/terms/Assertion
bdqffdq:Assertion rdf:type owl:Class ;
                  rdfs:subClassOf bdqffdq:ReportConcept ;
                  dcterms:issued "2024-09-30"^^xsd:date ;
                  rdfs:comment "The Assertion type in bdqffdq is the fundamental concept that makes up a data quality report. Assertion can be any one of four types (represented as subClasses), Measure, Validation, Issue, and Amendement.  The assertion concept consists of a Specification (the technical description of a performed test), a data resource (initial values of input data expressed in terms of some controlled vocabulary), the mechanism (external service, actor, or code that performs the test), and some form of result." ;
                  rdfs:label "Assertion"@en ;
                  skos:definition "A report concept expressing a statement about data quality assertion following some Specification produced by some implementation pertaining to some data resource." ;
                  skos:prefLabel "Assertion"@en .


###  https://rs.tdwg.org/bdqffdq/terms/Consulted
bdqffdq:Consulted rdf:type owl:Class ;
                  rdfs:subClassOf bdqffdq:InformationElement ;
                  dcterms:issued "2024-09-30"^^xsd:date ;
                  rdfs:comment "An InformationElement the content of which is examined to assert a result on one or more other InformationElements."@en ;
                  rdfs:label "Consulted"@en ;
                  skos:definition "An information element, expressed in concrete terms, about which a data quality need examines in order to expresses assertions about the data quality in another InformationElement." ;
                  skos:prefLabel "Acted Upon" .


###  https://rs.tdwg.org/bdqffdq/terms/Criterion
bdqffdq:Criterion rdf:type owl:Class ;
                  rdfs:subClassOf bdqffdq:FundamentalConcept ,
                                  bdqffdq:NeedConcept ;
                  dcterms:issued "2024-09-30"^^xsd:date ;
                  rdfs:comment "General statement, for example: In a controlled vocabulary.  Composed with both Validations and Issues."@en ;
                  rdfs:label "Criterion"@en ;
                  skos:definition "Rule against which data are evaluated for conformance to quality criteria."@en ;
                  skos:prefLabel "Criterion"@en .


###  https://rs.tdwg.org/bdqffdq/terms/DataQualityDimension
bdqffdq:DataQualityDimension rdf:type owl:Class ;
                             rdfs:subClassOf bdqffdq:FundamentalConcept ,
                                             bdqffdq:NeedConcept ;
                             dcterms:issued "2024-09-30"^^xsd:date ;
                             rdfs:comment "Describes the aspect of data quality (accuracy, precision, completeness, etc.) that a test examines. For example, [precision] in [coordinate precision of single records].  In the original framework only related to Measures, here may be related to any DataQualityNeed."@en ;
                             rdfs:label "Data Quality Dimension"@en ;
                             skos:definition "An aspect of data quality."@en ;
                             skos:prefLabel "Data Quality Dimension" .


###  https://rs.tdwg.org/bdqffdq/terms/DataQualityMethod
bdqffdq:DataQualityMethod rdf:type owl:Class ;
                          rdfs:subClassOf bdqffdq:SolutionsConcept ;
                          dcterms:issued "2024-09-30"^^xsd:date ;
                          rdfs:comment "DataQualityMethods are associative entities that allow Specifications or data quality tests to be reused by supporting a many to many relationship between the two." ;
                          rdfs:label "Data Quality Method"@en ;
                          skos:definition "A solutions concept that relates a data quality need to a Specification." ;
                          skos:prefLabel "Data Quality Method"@en .


###  https://rs.tdwg.org/bdqffdq/terms/DataQualityNeed
bdqffdq:DataQualityNeed rdf:type owl:Class ;
                        rdfs:subClassOf bdqffdq:NeedConcept ;
                        dcterms:issued "2024-09-30"^^xsd:date ;
                        rdfs:comment "Subtypes of DataQualityNeed are the Test Types.  Data Quality Need appoximates the informal concept of Test as used in BDQ Core." ;
                        rdfs:label "Data Quality Need"@en ;
                        skos:definition "A data quality need concept that expresses what assertions may be made about data with respect to fitness for use." ;
                        skos:prefLabel "Data Quality Need"@en .


###  https://rs.tdwg.org/bdqffdq/terms/DataQualityProfile
bdqffdq:DataQualityProfile rdf:type owl:Class ;
                           rdfs:subClassOf bdqffdq:NeedConcept ;
                           dcterms:issued "2024-09-30"^^xsd:date ;
                           rdfs:comment """Profile in bdqffdq is a data quality Needs level concept describing the UseCases that make up some data quality operation such as the behavior of a single actor or workflow producing the relevant assertions.  

DQP (u) = {dqp | dqp = mp(u) ⋃ vp(u) ⋃ ep(u), mp ∈ MP , vp ∈ VP , ep ∈ EP ⋀ u ∈ U }""" ;
                           rdfs:label "Data Quality Profile"@en ;
                           skos:definition "A needs concept expressing the composition of Policies to satisfy a UseCase." ;
                           skos:prefLabel "Data Quality Profile"@en .


###  https://rs.tdwg.org/bdqffdq/terms/DataQualityReport
bdqffdq:DataQualityReport rdf:type owl:Class ;
                          rdfs:subClassOf bdqffdq:ReportConcept ;
                          dcterms:issued "2024-09-30"^^xsd:date ;
                          rdfs:comment "The DataQualityReport concept consists of a set of assertions (MeasureAssertions, ValidationAssertions, IssueAssertions and AmendmentAssertions) that represent the output of a workflow/actor run.  These assertions form an account of the fitness for use of a tested data set for a specified use, as produced by a Mechanism."@en ;
                          rdfs:label "Data Quality Report"@en ;
                          skos:definition "A report concept comprising a set of data quality assertions." ;
                          skos:prefLabel "Data Quality Report"@en .


###  https://rs.tdwg.org/bdqffdq/terms/DataResource
bdqffdq:DataResource rdf:type owl:Class ;
                     rdfs:subClassOf bdqffdq:ReportConcept ;
                     dcterms:issued "2024-09-30"^^xsd:date ;
                     rdfs:comment """Describes a data resource containing terms from a controlled vocabulary such as (dwc) that can be related to information elements and represents the original values of the data operated on by an assertion test (i.e. an instance of dwc:Occurrence).  Ideally, DataResources have persistent GUIDs.

A data resource could be the oa:target of a oa:Annotation of which an Assertion is the oa:body.

DR = { dr | dr = < id, rt, v >, id ∈ I D, rt ∈ RT , (rt = sr ⋁ rt = ds) ⋀ v ∈ V }""" ;
                     rdfs:label "Data Resource"@en ;
                     skos:definition "A thing to whch a data quality assertion applies." ;
                     skos:prefLabel "Data Resource"@en .


###  https://rs.tdwg.org/bdqffdq/terms/Enhancement
bdqffdq:Enhancement rdf:type owl:Class ;
                    rdfs:subClassOf bdqffdq:AmendmentConcept ,
                                    bdqffdq:FundamentalConcept ,
                                    bdqffdq:NeedConcept ;
                    dcterms:issued "2024-09-30"^^xsd:date ;
                    rdfs:comment "General statement, for example: Recommend replacement value from a controlled vocabulary."@en ;
                    rdfs:label "Enhancement"@en ;
                    skos:definition "Description of a means by which data could be improved."@en ;
                    skos:prefLabel "Enhancement"@en .


###  https://rs.tdwg.org/bdqffdq/terms/FundamentalConcept
bdqffdq:FundamentalConcept rdf:type owl:Class ;
                           dcterms:issued "2024-09-30"^^xsd:date ;
                           rdfs:comment "Contrast with derived concepts, which are compositions of two or more fundamental concepts.  See Veiga et al., 2017.   Derived concepts can be organized by test type into AmendmentConcept, ValidationConcept, MeasurementConcept or IssueConcept.  Derived concepts can also be organized by framework layer into NeedsConcept, SolutionsConcept, and ReportConcept." ;
                           rdfs:label "Fundamental Concept"@en ;
                           skos:definition "Category of fitness for use concepts that are not derived by composition with other concepts."@en ;
                           skos:prefLabel "Fundamental Concept"@en .


###  https://rs.tdwg.org/bdqffdq/terms/Implementation
bdqffdq:Implementation rdf:type owl:Class ;
                       rdfs:subClassOf bdqffdq:SolutionsConcept ;
                       dcterms:issued "2024-09-30"^^xsd:date ;
                       rdfs:comment """The bdqffdq derived concept of an Implementation describes the relationship between a Specification (technical description of a test) and the mechanism that implements it.

I (s) = {m | m ⊂ M ⋀ s ∈ S}""" ;
                       rdfs:label "Implementation"@en ;
                       skos:definition "A solutions concept that describes the portion of a Mechanism that carries out the proccess described in a particular Specification." ;
                       skos:prefLabel "Implementation"@en .


###  https://rs.tdwg.org/bdqffdq/terms/ImprovementTarget
bdqffdq:ImprovementTarget rdf:type owl:Class ;
                          rdfs:subClassOf bdqffdq:NeedConcept ;
                          dcterms:issued "2024-09-30"^^xsd:date ;
                          rdfs:comment """The ImprovementTarget concept in bdqffdq describes which measures, issues, and validations are improved by some amendment. ImprovementTarget includes relationships between an Amendment and one or more Validations or Measures.

IT(am) = {me ⋃ va | me ∈ ME, va ∈ VA ⋀ am ∈ AM}"""@en ;
                          rdfs:label "Improvement Target"@en ;
                          skos:definition "A specific data quality need for which a specific Amendment is intended to improve." ;
                          skos:prefLabel "Improvement Target"@en .


###  https://rs.tdwg.org/bdqffdq/terms/InformationElement
bdqffdq:InformationElement rdf:type owl:Class ;
                           rdfs:subClassOf bdqffdq:FundamentalConcept ;
                           dcterms:issued "2024-09-30"^^xsd:date ;
                           rdfs:comment "An information element identifies a portion of data to which a test pertains.  The information element in bdqffdq can be represented as a single or composite element that consists of one or more terms from a controlled vocabulary (fields actedUpon or consulted by an assertion test) that identifies concepts in data relevant to a UseCase.  An abstraction or a concrete term that represents relevant content (e.g., coordinates; dwc.decimalLatitude, dwc:decimalLongitude)."@en ;
                           rdfs:label "Information Element"@en ;
                           skos:definition "A portion of data with which a Data Quality Need is concerned." ;
                           skos:prefLabel "Information Element"@en .


###  https://rs.tdwg.org/bdqffdq/terms/Issue
bdqffdq:Issue rdf:type owl:Class ;
              rdfs:subClassOf bdqffdq:DataQualityNeed ,
                              bdqffdq:IssueConcept ;
              dcterms:issued "2024-09-30"^^xsd:date ;
              rdfs:comment """Added to the original framework.  Inverse of Contextualized Criterion in the original framework.  Describes an instance of the issue concept in terms of the associated information elements from some controlled vocabulary (fields actedUpon or consulted), and a resource type of SingleRecord or MultiRecord.  Describes criteria by which data which lack quality for some purpose may be identified.  An issue is phrased in a negative sense, and approximates an inverse of a Validation.  An Issue identifies data that lack or may lack quality.  An Issue may flag a POTENTIAL_ISSUE that would need further review to determine if the data have quality for some purpose,  If the conditions described by an issue are identified by a test, the Problem Assertion result will be either IS_ISSUE or POTENTIAL_ISSUE, if no issue is found with the data the result will be NOT_ISSUE.  NOT_ISSUE, unlike COMPLIANT for a Validation, does not assert that data are fit for some purpose.    An Issue is the data quality needs concept that parallels a IssueMethod at the solutions level, and a IssueAssertion at the report level.   

IS = { is | is = < ie, c, rt >, ie ∈ IE, c ∈ ∁C ⋀ rt ∈ RT }"""@en ;
              rdfs:label "Issue"@en ;
              skos:definition "A data quality need that expresses how quality problems may be identified in data." ;
              skos:prefLabel "Issue"@en .


###  https://rs.tdwg.org/bdqffdq/terms/IssueAssertion
bdqffdq:IssueAssertion rdf:type owl:Class ;
                       rdfs:subClassOf bdqffdq:Assertion ,
                                       bdqffdq:IssueConcept ;
                       dcterms:issued "2024-09-30"^^xsd:date ;
                       rdfs:comment """The data quality report concept describing a the result of a test in the negative, that is identifying the potential absence of data quality. 

If a problem was found the ResponseResult is expected to carry a a value of IS_ISSUE, if a potential problem was found that needs human review the ResponseResult is expected to be of POTENTIAL_ISSUE, otherwise if the ResponseStatus is RUN_HAS_RESULT,  the ResponseResult is expected to be NOT_ISSUE.""" ;
                       rdfs:label "Issue Assertion"@en ;
                       skos:definition "An assertion expressing the result of an implementation evaluating an issue for a particular data quality need in a particular data resource." ;
                       skos:prefLabel "Issue Assertion"@en .


###  https://rs.tdwg.org/bdqffdq/terms/IssueConcept
bdqffdq:IssueConcept rdf:type owl:Class ;
                     dcterms:issued "2024-09-30"^^xsd:date ;
                     rdfs:comment "Issue terms are expressed in a negative sense, they identify data that do not or may not conform to quality needs."@en ;
                     rdfs:label "Issue Concept"@en ;
                     skos:definition "A term involved in flagging problems or potential problems in assessment of data quality that would or might prevent the data from meeting expressed data quality needs."@en ;
                     skos:prefLabel "Issue Concept"@en .


###  https://rs.tdwg.org/bdqffdq/terms/IssueMethod
bdqffdq:IssueMethod rdf:type owl:Class ;
                    rdfs:subClassOf bdqffdq:DataQualityMethod ,
                                    bdqffdq:IssueConcept ;
                    dcterms:issued "2024-09-30"^^xsd:date ;
                    rdfs:comment "The IssueMethod in bdqffdq is a data quality Solutions level concept describing the relationship between a Specification (technical description of a test) and an Issue (a Criterion in the context of resource type (SingleRecord or MultiRecord) and associated information elements)." ;
                    rdfs:label "Issue Method"@en ;
                    skos:definition "A data quality solution concept that relates an Issue to its Specifications." ;
                    skos:prefLabel "Issue Method"@en .


###  https://rs.tdwg.org/bdqffdq/terms/IssuePolicy
bdqffdq:IssuePolicy rdf:type owl:Class ;
                    rdfs:subClassOf bdqffdq:IssueConcept ,
                                    bdqffdq:Policy ;
                    dcterms:issued "2024-09-30"^^xsd:date ;
                    rdfs:comment "The IssuePolicy in bdqffdq is a data quality Needs level concept that describes how some Issue relates to a UseCase. This relationship defines which Issues are supported by a given UseCase." ;
                    rdfs:label "Issue Policy"@en ;
                    skos:definition "A need concept that relates a UseCase to a set of supporting Issues." ;
                    skos:prefLabel "Issue Policy"@en .


###  https://rs.tdwg.org/bdqffdq/terms/Measure
bdqffdq:Measure rdf:type owl:Class ;
                rdfs:subClassOf bdqffdq:DataQualityNeed ,
                                bdqffdq:MeasurementConcept ;
                dcterms:issued "2024-09-30"^^xsd:date ;
                rdfs:comment """Contextualized Dimension in the original framework Describes an instance of the measure concept in terms of the associated information elements from some controlled vocabulary (fields ActedUpon or Consulted), and a ResourceType of SingleRecord or MultiRecord. 

Describes the criteria for measuring an aspect of data quality related to some data quality need.   May be criteria for determining that data are COMPLETE or NOT_COMPLETE, or may be criteria for asserting a numeric measurement.  COMPLETE or NOT_COMPLETE measures are fundamental to data quality control, as set of data are filtered to the subset of data that have quality for some need if all records are COMPLETE for all pertenent Measures. 

A Measure is the data quality needs concept that parallels a MeasurementMethod at the solutions level, and a MeasurementAssertion at the report level.

ME = { me | me =< ie, d, rt >, ie ∈ IE, d ∈ D ⋀ rt ∈ RT }
also acceptable measure
AM(me) = {va | me ∈ C D ⋀ va ⊂ C C}"""@en ;
                rdfs:label "Measure"@en ;
                skos:definition "A data quality need that expresses how the fitness of data for some use may be measured." ;
                skos:prefLabel "Measure"@en .


###  https://rs.tdwg.org/bdqffdq/terms/MeasurementAssertion
bdqffdq:MeasurementAssertion rdf:type owl:Class ;
                             rdfs:subClassOf bdqffdq:Assertion ,
                                             bdqffdq:MeasurementConcept ;
                             dcterms:issued "2024-09-30"^^xsd:date ;
                             rdfs:comment """The MeasurementAssertion is a report level concept that describes the results of the execution of of a test that performs a MeasurementMethod following some Specification to assess some data quality Measurement. 

In bdqffdq, the MeasurementAssertion is expected to carry a ResponseResult of COMPLETE or NOT_COMPLETE or a numeric measured value value (e.g. a measure of dwc:eventDate duration in seconds).

DQM(dr) = {dqm | dqm =< me, s, m, r >, me ∈ ME, s ∈ S, m ∈ M , r ∈ R ⋀ dr ∈ DR}""" ;
                             rdfs:label "Measurement Assertion"@en ;
                             skos:definition "An assertion expressing the result of an implementation measuring a particular data quality need in a particular data resource." ;
                             skos:prefLabel "Measurement Assertion"@en .


###  https://rs.tdwg.org/bdqffdq/terms/MeasurementMethod
bdqffdq:MeasurementMethod rdf:type owl:Class ;
                          rdfs:subClassOf bdqffdq:DataQualityMethod ,
                                          bdqffdq:MeasurementConcept ;
                          dcterms:issued "2024-09-30"^^xsd:date ;
                          rdfs:comment """The MeasurementMethod in bdqffdq is a data quality Solutions level concept describing the relationship between a Specification (technical description of a test) and a Measurement (a dimension in the context of resource type (SingleRecord or MultiRecord) and associated information elements).

MM(me) = {s | s ⊂ S ⋀ me ∈ ME}""" ;
                          rdfs:label "Measurement Method"@en ;
                          skos:definition "A data quality solution concept that relates a Measure to its Specifications." ;
                          skos:prefLabel "Measurement Method"@en .


###  https://rs.tdwg.org/bdqffdq/terms/MeasurementPolicy
bdqffdq:MeasurementPolicy rdf:type owl:Class ;
                          rdfs:subClassOf bdqffdq:MeasurementConcept ,
                                          bdqffdq:Policy ;
                          dcterms:issued "2024-09-30"^^xsd:date ;
                          rdfs:comment """The MeasurementPolicy in bdqffdq is a data quality Needs level concept that describes how some Measurement relates to a UseCase. This relationship defines which measures are supported by a given UseCase.

MP(u) = {me | me ⊂ ME ⋀ u ∈ U }""" ;
                          rdfs:label "Measurement Policy"@en ;
                          skos:definition "A need concept that relates a UseCase to a set of supporting Measures." ;
                          skos:prefLabel "Measurement Policy"@en .


###  https://rs.tdwg.org/bdqffdq/terms/MeasurementConcept
bdqffdq:MeasurementConcept rdf:type owl:Class ;
                          dcterms:issued "2024-09-30"^^xsd:date ;
                          rdfs:label "Measurement Concept"@en ;
                          skos:definition "A term involved in measurement of data quality with regards to expressed data quality needs."@en ;
                          skos:prefLabel "Measurement Concept"@en .


###  https://rs.tdwg.org/bdqffdq/terms/Mechanism
bdqffdq:Mechanism rdf:type owl:Class ;
                  rdfs:subClassOf bdqffdq:FundamentalConcept ,
                                  bdqffdq:SolutionsConcept ;
                  dcterms:issued "2024-09-30"^^xsd:date ;
                  rdfs:comment """Mechanisms may produce data quality reports as products.    

The bdqffdq concept of mechanism describes the entity that performs an assertion test (code, external service, actor, etc.). Tied to a Specification via the concept of an Implementation.""" ;
                  rdfs:label "Mechanism"@en ;
                  skos:definition "An entity that can execute data quality methods."@en ;
                  skos:prefLabel "Mechanism"@en .


###  https://rs.tdwg.org/bdqffdq/terms/NeedConcept
bdqffdq:NeedConcept rdf:type owl:Class ;
                    dcterms:issued "2024-09-30"^^xsd:date ;
                    rdfs:comment "Category of concepts forming the Needs layer of the fitness for use framework." ;
                    rdfs:label "Need Concept"@en ;
                    skos:definition "A concept that expresses an aspect of a data quality need."@en ;
                    skos:prefLabel "Need Concept"@en .


###  https://rs.tdwg.org/bdqffdq/terms/Parameter
bdqffdq:Parameter rdf:type owl:Class ;
                  rdfs:subClassOf bdqffdq:SolutionsConcept ;
                  dcterms:issued "2024-09-30"^^xsd:date ;
                  rdfs:comment "A Parameter is a Formal Parameter for which an Argument is an Actual Parameter that replaces it to determine the behavior of a Specification.  An extension to the original fitness for use framework as described in Veiga et al., 2017." ;
                  rdfs:label "Parameter"@en ;
                  skos:definition "A placeholder for a value that, when provided to a test Specification changes the behavior of the test in a defined manner."@en ;
                  skos:prefLabel "Parameter"@en .


###  https://rs.tdwg.org/bdqffdq/terms/Policy
bdqffdq:Policy rdf:type owl:Class ;
               rdfs:subClassOf bdqffdq:NeedConcept ;
               dcterms:issued "2024-09-30"^^xsd:date ;
               rdfs:comment "Composition of data quality Needs into UseCases." ;
               rdfs:label "Policy" ;
               skos:definition "The set of data quality Needs for a UseCase" ;
               skos:prefLabel "Policy" .


###  https://rs.tdwg.org/bdqffdq/terms/ReportConcept
bdqffdq:ReportConcept rdf:type owl:Class ;
                      dcterms:issued "2024-09-30"^^xsd:date ;
                      rdfs:comment "Category of concepts forming the Report layer of the fitness for use framework."@en ;
                      rdfs:label "Report Concept" ;
                      skos:definition "A concept concerning data quality expressed in a data quality report." ;
                      skos:prefLabel "Report Concept"@en .


###  https://rs.tdwg.org/bdqffdq/terms/ResourceType
bdqffdq:ResourceType rdf:type owl:Class ;
                     rdfs:subClassOf bdqffdq:FundamentalConcept ;
                     dcterms:issued "2024-09-30"^^xsd:date ;
                     rdfs:comment "In bdqffdq the concept of ResourceType has instances for SingleRecord or MultiRecord." ;
                     rdfs:label "Resource Type"@en ;
                     skos:definition "Category of things that are data objects about which data quality assertions may be made." ;
                     skos:prefLabel "Resource Type"@en .


###  https://rs.tdwg.org/bdqffdq/terms/ResponseQualifier
bdqffdq:ResponseQualifier rdf:type owl:Class ;
                          rdfs:subClassOf bdqffdq:ReportConcept ;
                          dcterms:issued "2024-09-30"^^xsd:date ;
                          rdfs:comment "Intended as an extension point for qualifying information about uncertainty or ambiguity." ;
                          rdfs:label "Response Qualifier" ;
                          skos:definition "A report concept to which additional assertions providing additional information beyond that of ResponseResult from the result of the execution of the Specification of a data quality need are attached." ;
                          skos:prefLabel "Response Qualifier" .


###  https://rs.tdwg.org/bdqffdq/terms/ResponseResult
bdqffdq:ResponseResult rdf:type owl:Class ;
                       rdfs:subClassOf bdqffdq:ReportConcept ;
                       dcterms:issued "2024-09-30"^^xsd:date ;
                       rdfs:comment """For Validations, response results may be COMPLIANT, or NOT_COMPLIANT.  For Measures, response result objects may be COMPLETE or NOT_COMPLETE.  For Issues, Response results may be IS_ISSUE, POTENTIAL_ISSUE, or NOT_ISSUE.  See the bdq: vocabulary.  Measures may also use a numeric data property.  Amendments assert a string data property.

The report ResponseResult in bdqffdq is represented as a value or a result object for MeasureAsssertions, just a result object for ValidationAssertions and values for changes propsed in AmendmentAssertions.""" ;
                       rdfs:label "Response.result"@en ;
                       skos:definition "A report concept to which a controlled vocabulary assertions about the result of the execution of the Specification of a data quality need are attached." ;
                       skos:prefLabel "Response.result"@en .


###  https://rs.tdwg.org/bdqffdq/terms/ResponseStatus
bdqffdq:ResponseStatus rdf:type owl:Class ;
                       rdfs:subClassOf bdqffdq:ReportConcept ;
                       dcterms:issued "2024-09-30"^^xsd:date ;
                       rdfs:comment "The ResponseStatus is metadata, indicating if data should be present in a ResponseResult.   Any assertion may have the values INTERNAL_PREREQUISITES_NOT_MET of EXTERNAL_PREREQUISITES_NOT_MET, indicating that no value would be present in the accompanying ResponseResult.  Other values depend on the Assertion type.  Thes would be RUN_HAS_RESULT for a Validation, Measure, or Isssue, and, FILLED_IN, AMENDED, or NOT_AMENDED for an Amendment.  Additional metadata qualifying the assertion in a ReqponseResult, such as statements of uncertainy or ambiguity may be placed in the ResponseQualifier." ;
                       rdfs:label "Response.status"@en ;
                       skos:definition "A report concept expressing controlled vocabulary values about the exit state of an execution process of a data quality Specification by an implementation." ;
                       skos:prefLabel "Response.status"@en .


###  https://rs.tdwg.org/bdqffdq/terms/SolutionsConcept
bdqffdq:SolutionsConcept rdf:type owl:Class ;
                         dcterms:issued "2024-09-30"^^xsd:date ;
                         rdfs:comment "Category of concepts forming the Solutions layer of the fitness for use framework.  Solutions are tools that evaluate data against needs and express conclusions in data quality reports."@en ;
                         rdfs:label "Solutions Concept"@en ;
                         skos:definition "A concept that expresses an aspect of a data quality solution." ;
                         skos:prefLabel "Solutions Concept"@en .


###  https://rs.tdwg.org/bdqffdq/terms/Specification
bdqffdq:Specification rdf:type owl:Class ;
                      rdfs:subClassOf bdqffdq:FundamentalConcept ,
                                      bdqffdq:SolutionsConcept ;
                      dcterms:issued "2024-09-30"^^xsd:date ;
                      rdfs:comment "A Specification is a technical desription of an assertion test.  A Specification is expected to have the following properies:  (1) Expected Response, (2) Authorities and Parameters."@en ;
                      rdfs:label "Specification"@en ;
                      skos:definition "A specific statement about how to evaluate a data quality need."@en ;
                      skos:prefLabel "Specification"@en .


###  https://rs.tdwg.org/bdqffdq/terms/UseCase
bdqffdq:UseCase rdf:type owl:Class ;
                rdfs:subClassOf bdqffdq:FundamentalConcept ,
                                bdqffdq:NeedConcept ;
                dcterms:issued "2024-09-30"^^xsd:date ;
                rdfs:comment "The UseCase concept in bdqffdq describes some data quality control UseCase. The Amendment, Measurement and Validation policies that make up a UseCase define which assertions cover a given UseCase.  An example of a UseCase could be \"Check for internal consistency of dates\", with validation policies for checking consistency between atomic date fields and an Amendment such as \"eventDate filled in from verbatim\".  UseCases in bdqffdq are not the same as UseCases in the software engineering sense, but are similar bdqffdq formal statements derived from analyis of user stories." ;
                rdfs:label "Use Case"@en ;
                skos:definition "A needs concept expressing a purpose to which data are put for which the data must have quality for the result to have meaning and reliability." ;
                skos:prefLabel "Use Case"@en .


###  https://rs.tdwg.org/bdqffdq/terms/Validation
bdqffdq:Validation rdf:type owl:Class ;
                   rdfs:subClassOf bdqffdq:DataQualityNeed ,
                                   bdqffdq:ValidationConcept ;
                   dcterms:issued "2024-09-30"^^xsd:date ;
                   rdfs:comment """ContextualizedCriterion in the original framework.  Describes the criteria for determining compliance of data to fill some data quality need.  A description of a criterion applied to an information element for some resource type.   Describes an instance of the criterion concept in terms of the associated information elements from some controlled vocabulary (fields actedUpon or consulted), and a resource type of SingleRecord or MultiRecord.  

Validations are phrased in a positive sense, they identify data which has quality for some need.  For example: The value of basisOfRecord of single records must be in the controlled vocabulary.   

A Validation is the data quality needs concept that parallels a ValidationMethod at the solutions level, and a ValidationAssertion at the report level.  ValidationAssertions may specify a result that is COMPLIANT, where the data has quality, or NOT_COMPLIANT, where the data lacks quality for some use.  

VA = { va | va = < ie, c, rt >, ie ∈ IE, c ∈ C ⋀ rt ∈ RT }"""@en ;
                   rdfs:label "Validation"@en ;
                   skos:definition "A data quality need that expreses how data may be evaluated for fitness for use."@en ;
                   skos:prefLabel "Validation"@en .


###  https://rs.tdwg.org/bdqffdq/terms/ValidationAssertion
bdqffdq:ValidationAssertion rdf:type owl:Class ;
                            rdfs:subClassOf bdqffdq:Assertion ,
                                            bdqffdq:ValidationConcept ;
                            dcterms:issued "2024-09-30"^^xsd:date ;
                            rdfs:comment """The ValidationAssertion is a report level concept that describes the results of the execution of of a test that performs a ValidationMethod following some Specification to assess the validity of some data with respect to the Criteria of some Validation. 

The ValidationAssertion concept in bdqffdq is expected to carry a a ResponseResult of COMPLIANT or NON_COMPLIANT.

DQV(dr) = {dqv | dqv = < va, s, m, r >, va ∈ VA, s ∈ S, m ∈ M , r ∈ R ⋀ dr ∈ DR}""" ;
                            rdfs:label "Validation Assertion"@en ;
                            skos:definition "An assertion expressing the result of an implementation validating compliance with a a particular data quality need in a particular data resource." ;
                            skos:prefLabel "Validation Assertion"@en .


###  https://rs.tdwg.org/bdqffdq/terms/ValidationConcept
bdqffdq:ValidationConcept rdf:type owl:Class ;
                          dcterms:issued "2024-09-30"^^xsd:date ;
                          rdfs:comment "Validation terms are expressed in a positive sense, they identify data that conform to needs."@en ;
                          rdfs:label "Validation Concept"@en ;
                          skos:definition "A term involved in statements about the conformance of data to expressed quality needs."@en ;
                          skos:prefLabel "Validation Concept"@en .


###  https://rs.tdwg.org/bdqffdq/terms/ValidationMethod
bdqffdq:ValidationMethod rdf:type owl:Class ;
                         rdfs:subClassOf bdqffdq:DataQualityMethod ,
                                         bdqffdq:ValidationConcept ;
                         dcterms:issued "2024-09-30"^^xsd:date ;
                         rdfs:comment """The ValidationMethod in bdqffdq is a data quality Solutions level concept describing the relationship between a Specification (technical description of a test) and a Validation (a Criterion in the context of resource type (SingleRecord or MultiRecord) and associated information elements).

VM(va) = {s | s ⊂ S ⋀ va ∈ VA}""" ;
                         rdfs:label "Validation Method"@en ;
                         skos:definition "A data quality solution concept that relates an Validation to its Specifications." ;
                         skos:prefLabel "Validation Method"@en .


###  https://rs.tdwg.org/bdqffdq/terms/ValidationPolicy
bdqffdq:ValidationPolicy rdf:type owl:Class ;
                         rdfs:subClassOf bdqffdq:Policy ,
                                         bdqffdq:ValidationConcept ;
                         dcterms:issued "2024-09-30"^^xsd:date ;
                         rdfs:comment """The ValidationPolicy in bdqffdq is a data quality Needs level concept that describes how some Validation relates to a UseCase. This relationship defines which Validations are needed to identify quality in a given UseCase.

VP (u) = {va | va ⊂ VA ⋀ u ∈ U }""" ;
                         rdfs:label "Validation Policy"@en ;
                         skos:definition "A need concept that relates a UseCase to a set of supporting Validations." ;
                         skos:prefLabel "Validation Policy"@en .


#################################################################
#    Individuals
#################################################################

###  https://rs.tdwg.org/bdqffdq/terms/AMENDED
bdqffdq:AMENDED rdf:type owl:NamedIndividual ,
                         bdqffdq:ResponseStatus ;
                owl:differentFrom bdqffdq:NOT_AMENDED ;
                dcterms:issued "2024-09-30"^^xsd:date ;
                rdf:value "AMENDED" ;
                rdfs:comment "AMENDED implies that a change is being proposed to some existing non-empty value.  Amendments do not provide bdqffdq:hasResponseResult object properties.  Proposed changes will be in a bdqffdq:hasResponseResultValue data property." ;
                rdfs:label "AMENDED" ;
                skos:definition "A bdqffdq:ResponseStatus used to indicate that a bdqffdq:hasResponseResultValue from a bdqffdq:Amendment contains a proposed change." ;
                skos:prefLabel "AMENDED" .


###  https://rs.tdwg.org/bdqffdq/terms/COMPLETE
bdqffdq:COMPLETE rdf:type owl:NamedIndividual ,
                          bdqffdq:ResponseResult ;
                 owl:differentFrom bdqffdq:NOT_COMPLETE ;
                 dcterms:issued "2024-09-30"^^xsd:date ;
                 rdf:value "COMPLETE" ;
                 rdfs:comment "These can be used to include data for Quality Assurance.  These can be asserted, for example by bdqffdq:Measures of bdqffdq:MultiRecords where all the bdqffdq:Validation bdqffdq:ResponseResult from all included records in the dataset are bdqffdq:COMPLIANT." ;
                 rdfs:label "COMPLETE" ;
                 skos:definition "A bdqffdq:ResponseResult of a bdqffdq:Measure which asserts that data are present and sufficiently comprehensive for use." ;
                 skos:prefLabel "COMPLETE" .


###  https://rs.tdwg.org/bdqffdq/terms/COMPLIANT
bdqffdq:COMPLIANT rdf:type owl:NamedIndividual ,
                           bdqffdq:ResponseResult ;
                  owl:differentFrom bdqffdq:NOT_COMPLIANT ;
                  dcterms:issued "2024-09-30"^^xsd:date ;
                  rdf:value "COMPLIANT" ;
                  rdfs:label "COMPLIANT" ;
                  skos:definition "A bdqffdq:ResponseResult of a bdqffdq:Validation where the data conforms to the criteria for quality in the test specification." ;
                  skos:prefLabel "COMPLIANT" .


###  https://rs.tdwg.org/bdqffdq/terms/EXTERNAL_PREREQUISITES_NOT_MET
bdqffdq:EXTERNAL_PREREQUISITES_NOT_MET rdf:type owl:NamedIndividual ,
                                                bdqffdq:ResponseStatus ;
                                       owl:differentFrom bdqffdq:INTERNAL_PREREQUISITES_NOT_MET ;
                                       dcterms:issued "2024-09-30"^^xsd:date ;
                                       rdf:value "EXTERNAL_PREREQUISITES_NOT_MET" ;
                                       rdfs:label "EXTERNAL_PREREQUISITES_NOT_MET" ;
                                       skos:definition "A bdqffdq:ResponseStatus used to indicate that a bdqffdq:ResponseResult was not generated because a bdq:sourceAuthority was not available or was off-line. If the test is run at a later time, it may produce a different result." ;
                                       skos:prefLabel "EXTERNAL_PREREQUISITES_NOT_MET" .


###  https://rs.tdwg.org/bdqffdq/terms/FILLED_IN
bdqffdq:FILLED_IN rdf:type owl:NamedIndividual ,
                           bdqffdq:ResponseStatus ;
                  owl:differentFrom bdqffdq:NOT_AMENDED ;
                  dcterms:issued "2024-09-30"^^xsd:date ;
                  rdf:value "FILLED_IN" ;
                  rdfs:label "FILLED_IN" ;
                  skos:definition "A bdqffdq:ResponseStatus used to indicate that a bdqffdq:Amendment contains a proposed change to a record in a bdqffdq:hasResponseResultValue where the bdqffdq:InformationElement was bdq:Empty." ;
                  skos:prefLabel "FILLED_IN" .


###  https://rs.tdwg.org/bdqffdq/terms/INTERNAL_PREREQUISITES_NOT_MET
bdqffdq:INTERNAL_PREREQUISITES_NOT_MET rdf:type owl:NamedIndividual ,
                                                bdqffdq:ResponseStatus ;
                                       dcterms:issued "2024-09-30"^^xsd:date ;
                                       rdf:value "INTERNAL_PREREQUISITES_NOT_MET" ;
                                       rdfs:label "INTERNAL_PREREQUISITES_NOT_MET" ;
                                       skos:definition "A bdqffdq:ResponseStatus used to indicate that a bdqffdq:ResponseResult was not generated because values of the bdqffdq:InformationElement were insufficient to run the test. If the test is run at a later time on unmodified data, it should produce the same bdqffdq:Response." ;
                                       skos:prefLabel "INTERNAL_PREREQUISITES_NOT_MET" .


###  https://rs.tdwg.org/bdqffdq/terms/IS_ISSUE
bdqffdq:IS_ISSUE rdf:type owl:NamedIndividual ,
                          bdqffdq:ResponseResult ;
                 owl:differentFrom bdqffdq:NOT_ISSUE ,
                                   bdqffdq:POTENTIAL_ISSUE ;
                 dcterms:issued "2024-09-30"^^xsd:date ;
                 rdf:value "IS_ISSUE" ;
                 rdfs:comment "This is a parallel assertion to NOT_COMPLIANT" ;
                 rdfs:label "IS_ISSUE" ;
                 skos:definition "A bdqffdq:ResponseResult of a bdqffdq:Issue that flags where the data do not have sufficient quality for a use." ;
                 skos:prefLabel "IS_ISSUE" .


###  https://rs.tdwg.org/bdqffdq/terms/MultiRecord
bdqffdq:MultiRecord rdf:type owl:NamedIndividual ,
                             bdqffdq:ResourceType ;
                    dcterms:issued "2024-09-30"^^xsd:date ;
                    rdfs:comment "A data set.  Encoded data with a defined structure that can be described as dcmitype:Dataset." ;
                    rdfs:label "Multi Record"@en ;
                    skos:definition "A set of one or more Single Records." ;
                    skos:prefLabel "Multi Record" .


###  https://rs.tdwg.org/bdqffdq/terms/NOT_AMENDED
bdqffdq:NOT_AMENDED rdf:type owl:NamedIndividual ,
                             bdqffdq:ResponseStatus ;
                    dcterms:issued "2024-09-30"^^xsd:date ;
                    rdf:value "NOT_AMENDED" ;
                    rdfs:comment "No assertion will be provided in a bdqfdq:hasResponseResultValue.  Amendments do not provide bdqffdq:hasResponseResult object properties." ;
                    rdfs:label "NOT_AMENDED" ;
                    skos:definition "A bdqffdq:ResponseStatus used to indicate that a bdqffdq:Amendment proposed no change." ;
                    skos:prefLabel "NOT_AMENDED" .


###  https://rs.tdwg.org/bdqffdq/terms/NOT_COMPLETE
bdqffdq:NOT_COMPLETE rdf:type owl:NamedIndividual ,
                              bdqffdq:ResponseResult ;
                     dcterms:issued "2024-09-30"^^xsd:date ;
                     rdf:value "NOT_COMPLETE" ;
                     rdfs:comment "These can be used to exclude data for Quality Assurance.  These can be asserted, for example by bdqffdq:Measures of bdqffdq:MultiRecords where not all the bdqffdq:Validation bdqffdq:ResponseResult from all included records in the dataset are bdqffdq:COMPLIANT." ;
                     rdfs:label "NOT_COMPLETE" ;
                     skos:definition "A bdqffdq:ResponseResult of a bdqffdq:Measure which asserts that data are not present or are not sufficiently comprehensive for use." ;
                     skos:prefLabel "NOT_COMPLETE" .


###  https://rs.tdwg.org/bdqffdq/terms/NOT_COMPLIANT
bdqffdq:NOT_COMPLIANT rdf:type owl:NamedIndividual ,
                               bdqffdq:ResponseResult ;
                      dcterms:issued "2024-09-30"^^xsd:date ;
                      rdf:value "NOT_COMPLIANT" ;
                      rdfs:label "NOT_COMPLIANT" ;
                      skos:definition "A bdqffdq:ResponseResult of a bdqffdq:Validation where the data do not conform to the criteria for quality in the test specification." ;
                      skos:prefLabel "NOT_COMPLIANT" .


###  https://rs.tdwg.org/bdqffdq/terms/NOT_ISSUE
bdqffdq:NOT_ISSUE rdf:type owl:NamedIndividual ,
                           bdqffdq:ResponseResult ;
                  owl:differentFrom bdqffdq:POTENTIAL_ISSUE ;
                  dcterms:issued "2024-09-30"^^xsd:date ;
                  rdf:value "NOT_ISSUE" ;
                  rdfs:comment "This is similar to, but has different semantics to, bdqffdq:COMPLIANT for a bdqffdq:Validation.  COMPLIANT means that the data were evaluated as having quality according to some Criterion.  NOT_ISSUE means that no issue with data quality was found under some criterion for identifying the absence of quality." ;
                  rdfs:label "NOT_ISSUE" ;
                  skos:definition "A bdqffdq:ResponseResult of a bdqffdq:Issue where no potential problems were detected." ;
                  skos:prefLabel "NOT_ISSUE" .


###  https://rs.tdwg.org/bdqffdq/terms/POTENTIAL_ISSUE
bdqffdq:POTENTIAL_ISSUE rdf:type owl:NamedIndividual ,
                                 bdqffdq:ResponseResult ;
                        dcterms:issued "2024-09-30"^^xsd:date ;
                        rdf:value "POTENTIAL_ISSUE" ;
                        rdfs:comment "See also bdqffdq:IS_ISSUE and bdqffdq:NOT_ISSUE.  POTENTIAL_ISSUE has no analog in a bdqffdq:Validation." ;
                        rdfs:label "POTENTIAL_ISSUE" ;
                        skos:definition "A bdqffdq:ResponseResult of a bdqffdq:Issue that flags where the data may not have sufficient quality for a use.  The user will need to evaluate if the data is fit for their particular use or not." ;
                        skos:prefLabel "POTENTIAL_ISSUE" .


###  https://rs.tdwg.org/bdqffdq/terms/RUN_HAS_RESULT
bdqffdq:RUN_HAS_RESULT rdf:type owl:NamedIndividual ,
                                bdqffdq:ResponseStatus ;
                       dcterms:issued "2024-09-30"^^xsd:date ;
                       rdf:value "RUN_HAS_RESULT" ;
                       rdfs:comment "Applies to bdqffdq:Validations, bdqfdfq:Measures, and bdqffdq:Issues, but not bdqffdq:Amendments.   For Validations and Issues, the value will be found as a bdqffdq:ResponseResult object by following bdqffdq:hasResponseResult.  For Measures, the value could be either in the data property bdqffdq:hasResponseResultValue or could be a ResponseResult object." ;
                       rdfs:label "RUN_HAS_RESULT" ;
                       skos:definition "A bdqffdq:ResponseStatus used to indicate that that a result was correctly generated." ;
                       skos:prefLabel "RUN_HAS_RESULT" .


###  https://rs.tdwg.org/bdqffdq/terms/SingleRecord
bdqffdq:SingleRecord rdf:type owl:NamedIndividual ,
                              bdqffdq:ResourceType ;
                     dcterms:issued "2024-09-30"^^xsd:date ;
                     rdfs:comment """A record from a dataset.  May be a a database tuple in the strict sense, that is a single row in a table, or may be rows related across several tables, or a graph of data.   A SingleRecord is Single in that it has one instance of a core concept from the perspective of information elements assessed for a UseCase.  For example, in a use case where occurences are central, a SingleRecord would represent a single occurrence, but could have multiple identifications and multiple taxa related to it in a graph or data structure.  However, in a UseCase where taxa are central, a SingleRecord would represent a single Taxon entity (and might have multiple occurrences related to it as part of the SingleRecord, so long as the graph was limited before reaching other Taxon entities).

A SingleRecord, like a MultiRecord, is Encoded data with a defined structure that can be described as dcmitype:Dataset"""@en ;
                     rdfs:label "Single Record"@en ;
                     skos:definition "A single entity comprised of encoded data with a defined structure that contains one instance of a core concept from the perspective of information elements assessed for a data quality need." ;
                     skos:prefLabel "Single Record" .


#################################################################
#    General axioms
#################################################################

[ rdf:type owl:AllDisjointClasses ;
  owl:members ( bdqffdq:AbstractInformationElement
                bdqffdq:ActedUpon
                bdqffdq:Consulted
              )
] .


[ rdf:type owl:AllDisjointClasses ;
  owl:members ( bdqffdq:Amendment
                bdqffdq:Issue
                bdqffdq:Measure
                bdqffdq:Validation
              )
] .


###  Generated by the OWL API (version 4.5.29.2024-05-13T12:11:03Z) https://github.com/owlcs/owlapi
