@prefix : <https://rs.tdwg.org/bdqffdq/terms#> .
@prefix owl: <http://www.w3.org/2002/07/owl#> .
@prefix rdf: <http://www.w3.org/1999/02/22-rdf-syntax-ns#> .
@prefix xml: <http://www.w3.org/XML/1998/namespace> .
@prefix xsd: <http://www.w3.org/2001/XMLSchema#> .
@prefix rdfs: <http://www.w3.org/2000/01/rdf-schema#> .
@prefix skos: <http://www.w3.org/2004/02/skos/core#> .
@prefix bdqffdq: <https://rs.tdwg.org/bdqffdq/terms/> .
@prefix dcterms: <http://purl.org/dc/terms/> .
@base <https://rs.tdwg.org/bdqffdq/terms#> .

<https://rs.tdwg.org/bdqffdq/terms> rdf:type owl:Ontology ;
                                     owl:versionIRI <https://rs.tdwg.org/bdqffdq/terms/1.0> ;
                                     rdfs:comment "The classes and object properties found in this ontology are dedicated to fundamental and derived concepts from the Fitness For Use Framework described in the paper by Veiga et al., available at: http://journals.plos.org/plosone/article?id=10.1371/journal.pone.0178731 as modified to describe data quality fitness for use Tests in the TDWG BDQ Standard."@en ;
                                     rdfs:label "Biodiversity Data Quality Fitness for Use Framework (Ontology)"@en .

#################################################################
#    Annotation properties
#################################################################

###  http://purl.org/dc/terms/issued
dcterms:issued rdf:type owl:AnnotationProperty .


###  http://www.w3.org/1999/02/22-rdf-syntax-ns#value
rdf:value rdf:type owl:AnnotationProperty .


###  http://www.w3.org/2004/02/skos/core#definition
skos:definition rdf:type owl:AnnotationProperty .


###  http://www.w3.org/2004/02/skos/core#prefLabel
skos:prefLabel rdf:type owl:AnnotationProperty .


#################################################################
#    Datatypes
#################################################################

###  http://www.w3.org/2001/XMLSchema#date
xsd:date rdf:type rdfs:Datatype .


#################################################################
#    Object Properties
#################################################################

###  https://rs.tdwg.org/bdqffdq/terms/amendmentProperty
bdqffdq:amendmentProperty rdf:type owl:ObjectProperty ;
                          dcterms:issued "2024-09-30"^^xsd:date ;
                          rdfs:comment "Subproperties of this type group object properties that apply to bdqffdq:AmendmentConcepts such as bdqffdq:AmendmentPolicy (bdqffdq:DataQualityNeed), bdqffdq:AmendmentMethod (bdqffdq:DataQualityMethod) and bdqffdq:Amendment (bdqffdq:DataQualityReports)."@en ;
                          rdfs:label "amendment Property"@en ;
                          skos:definition "Category of object properties that apply to bdqffdq:Amendments" ;
                          skos:prefLabel "amendment Property"@en .


###  https://rs.tdwg.org/bdqffdq/terms/appliesTo
bdqffdq:appliesTo rdf:type owl:ObjectProperty ;
                  dcterms:issued "2024-09-30"^^xsd:date ;
                  rdfs:comment "If a bdqffdq:Assertion forms the oa:body of an oa:Annotation, the bdqffdq:appliesTo bdqffdq:DataResource would be the oa:target of the bdqffdq:Annotation. If bdqffdq:Assertions are composed in bdqffdq:DataQualityReports, the bdqffdq:appliesTo bdqffdq:DataResource is an item examined as part of the bdqffdq:DataQualityReport. Expectation for bdqffdq:SingleRecord Test bdqffdq:Assertions on Darwin Core data in the BDQ standard is that bdqffdq:appliesTo would point at a dwc:Occurrence record."@en ;
                  rdfs:label "applies To"@en ;
                  skos:definition "Describes the bdqffdq:DataResource about which a bdqffdq:Assertion is made."@en ;
                  skos:prefLabel "applies To"@en .


###  https://rs.tdwg.org/bdqffdq/terms/composedOf
bdqffdq:composedOf rdf:type owl:ObjectProperty ;
                   dcterms:issued "2024-09-30"^^xsd:date ;
                   rdfs:comment "Describes the properties from a controlled vocabulary that compose an InformationElement. For example, an InformationElement may be composedOf properties such as dwc:day, dwc:month and dwc:year."@en ;
                   rdfs:label "composed Of"@en ;
                   skos:definition "Specific vocabulary term that comprises a bdqffdq:InformationElement that is not a bdqffdq:AbstractInformationElement."@en ;
                   skos:prefLabel "composed Of"@en .


###  https://rs.tdwg.org/bdqffdq/terms/containsAssertion
bdqffdq:containsAssertion rdf:type owl:ObjectProperty ;
                          dcterms:issued "2024-09-30"^^xsd:date ;
                          rdfs:comment "Connects bdqffdq:Assertions together into bdqffdq:DataQualityReports. Alternatively, bdqffdq:Assertions can be contained in oa:Annotations, in which case this property is not used."@en ;
                          rdfs:label "contains Assertion"@en ;
                          skos:definition "Connects a bdqffdq:DataQualityReport with bdqffdq:Assertions that comprise that bdqffdq:DataQualityReport."@en ;
                          skos:prefLabel "contains Assertion"@en .


###  https://rs.tdwg.org/bdqffdq/terms/forAmendment
bdqffdq:forAmendment rdf:type owl:ObjectProperty ;
                     rdfs:subPropertyOf bdqffdq:amendmentProperty ,
                                        bdqffdq:forDataQualityNeed ;
                     rdfs:range [ rdf:type owl:Restriction ;
                                  owl:onProperty bdqffdq:forAmendment ;
                                  owl:someValuesFrom bdqffdq:Amendment
                                ] ;
                     dcterms:issued "2024-09-30"^^xsd:date ;
                     rdfs:comment "Use to link a bdqffdq:AmendmentMethod to a bdqffdq:Amendment. Describes the relationship between a bdqffdq:AmendmentMethod (Solutions layer, see Figure 3 in Veiga et al., 2017) and a bdqffdq:Amendment (Need layer, see Figure 3 in Veiga et al., 2017)."@en ;
                     rdfs:label "for Amendment"@en ;
                     skos:definition "Relates a bdqffdq:AmendmentMethod to a bdqffdq:Amendment."@en ;
                     skos:prefLabel "for Amendment"@en .


###  https://rs.tdwg.org/bdqffdq/terms/forDataQualityNeed
bdqffdq:forDataQualityNeed rdf:type owl:ObjectProperty ;
                           dcterms:issued "2024-09-30"^^xsd:date ;
                           rdfs:comment "Category of properties that link Tests to their bdqffdq:Methods."@en ;
                           rdfs:label "for Data Quality Need"@en ;
                           skos:definition "Category of properties that relates a bdqffdq:DataQualityNeed to specific bdqffdq:Methods."@en ;
                           skos:prefLabel "for Data Quality Need"@en .


###  https://rs.tdwg.org/bdqffdq/terms/forIssue
bdqffdq:forIssue rdf:type owl:ObjectProperty ;
                 rdfs:subPropertyOf bdqffdq:forDataQualityNeed ,
                                    bdqffdq:issueProperty ;
                 rdfs:range [ rdf:type owl:Restriction ;
                              owl:onProperty bdqffdq:forIssue ;
                              owl:someValuesFrom bdqffdq:Issue
                            ] ;
                 dcterms:issued "2024-09-30"^^xsd:date ;
                 rdfs:comment "Use to link a bdqffdq:IssueMethod to a bdqffdq:Issue. Describes the relationship between a bdqffdq:IssueMethod (Solutions layer, see Figure 3 in Veiga et al., 2017) and a bdqffdq:Issue (Need layer, see Figure 3 in Veiga et al., 2017). Parallel concepts are bdqffdq:forAmendment, bdqffdq:forValidation, and bdqffdq:forMeasure."@en ;
                 rdfs:label "for Issue"@en ;
                 skos:definition "Relates a bdqffdq:IssueMethod to a bdqffdq:Issue."@en ;
                 skos:prefLabel "for Issue"@en .


###  https://rs.tdwg.org/bdqffdq/terms/forMeasure
bdqffdq:forMeasure rdf:type owl:ObjectProperty ;
                   rdfs:subPropertyOf bdqffdq:forDataQualityNeed ,
                                      bdqffdq:measurementProperty ;
                   rdfs:range [ rdf:type owl:Restriction ;
                                owl:onProperty bdqffdq:forMeasure ;
                                owl:someValuesFrom bdqffdq:Measure
                              ] ;
                   dcterms:issued "2024-09-30"^^xsd:date ;
                   rdfs:comment "Use to link bdqffdq:MeasurementMethods (Solutions layer, see Figure 3 in Veiga et al., 2017) to bdqffdq:Measures (Need layer, see Figure 3 in Veiga et al., 2017). Parallel concepts are bdqffdq:forAmendment, bdqffdq:forValidation, and bdqffdq:forIssue."@en ;
                   rdfs:label "for Measure"@en ;
                   skos:definition "Relates a bdqffdq:MeasurementMethod to a bdqffdq:Measure."@en ;
                   skos:prefLabel "for Measure"@en .


###  https://rs.tdwg.org/bdqffdq/terms/forValidation
bdqffdq:forValidation rdf:type owl:ObjectProperty ;
                      rdfs:subPropertyOf bdqffdq:forDataQualityNeed ,
                                         bdqffdq:validationProperty ;
                      rdfs:range [ rdf:type owl:Restriction ;
                                   owl:onProperty bdqffdq:forValidation ;
                                   owl:someValuesFrom bdqffdq:Validation
                                 ] ;
                      dcterms:issued "2024-09-30"^^xsd:date ;
                      rdfs:comment "Use to link bdqffdq:ValidationMethods to bdqffdq:Validations. Describes the relationship between a bdqffdq:ValidationMethod (Solutions layer, see Figure 3 in Veiga et al., 2017) and a bdqffdq:Validation (Need layer, see Figure 3 in Veiga et al., 2017). Parallel concepts are bdqffdq:forAmendment, bdqffdq:forMeasure, and bdqffdq:forIssue."@en ;
                      rdfs:label "for Validation"@en ;
                      skos:definition "Relates a bdqffdq:ValidationMethod to a bdqffdq:Validation."@en ;
                      skos:prefLabel "for Validation"@en .


###  https://rs.tdwg.org/bdqffdq/terms/hasActedUponInformationElement
bdqffdq:hasActedUponInformationElement rdf:type owl:ObjectProperty ;
                                       rdfs:subPropertyOf bdqffdq:hasInformationElement ;
                                       dcterms:issued "2024-09-30"^^xsd:date ;
                                       rdfs:comment "Provides a relationship between bdqffdq: concepts and the bdqffdq:InformationElements that are bdqffdq:ActedUpon in a Test."@en ;
                                       rdfs:label "has Acted Upon Information Element"@en ;
                                       skos:definition "Describes the bdqffdq:ActedUpon bdqffdq:InformationElements assessed by a bdqffdq:DataQualityNeed about which bdqffdq:Assertions arising from the bdqffdq:DataQualityNeed would apply."@en ;
                                       skos:prefLabel "has Acted Upon Information Element"@en .


###  https://rs.tdwg.org/bdqffdq/terms/hasArgument
bdqffdq:hasArgument rdf:type owl:ObjectProperty ;
                    rdfs:range bdqffdq:Argument ;
                    dcterms:issued "2024-09-30"^^xsd:date ;
                    rdfs:comment "Expected to be a relationship between a bdqffdq:Specification and a bdqffdq:Argument, where the bdqffdq:Argument provides a value for a bdqffdq:Parameter (e.g., bdq:sourceAuthority), and a bdqffdq:hasAuthoritiesDefaults for the bdqffdq:Specification may provide a default value for the bdqffdq:Parameter under that bdqffdq:Specification."@en ;
                    rdfs:label "has Argument"@en ;
                    skos:definition "Relates a bdqffdq:Specification to a bdqffdq:Argument"@en ;
                    skos:prefLabel "has Argument"@en .


###  https://rs.tdwg.org/bdqffdq/terms/hasConsultedInformationElement
bdqffdq:hasConsultedInformationElement rdf:type owl:ObjectProperty ;
                                       rdfs:subPropertyOf bdqffdq:hasInformationElement ;
                                       dcterms:issued "2024-09-30"^^xsd:date ;
                                       rdfs:comment "Provides a relationship between bdqffdq: concepts and the bdqffdq:InformationElements that are bdqffdq:Consulted, but not bdqffdq:ActedUpon in a Test."@en ;
                                       rdfs:label "has Consulted Information Element"@en ;
                                       skos:definition "Describes the bdqffdq:InformationElements assessed by a bdqffdq:DataQualityNeed in order to make bdqffdq:Assertions concerning bdqffdq:ActedUpon bdqffdq:InformationElements."@en ;
                                       skos:prefLabel "has Consulted Information Element"@en .


###  https://rs.tdwg.org/bdqffdq/terms/hasCriterion
bdqffdq:hasCriterion rdf:type owl:ObjectProperty ;
                     rdfs:subPropertyOf bdqffdq:issueProperty ,
                                        bdqffdq:validationProperty ;
                     rdfs:range [ rdf:type owl:Restriction ;
                                  owl:onProperty bdqffdq:hasCriterion ;
                                  owl:someValuesFrom bdqffdq:Criterion
                                ] ;
                     dcterms:issued "2024-09-30"^^xsd:date ;
                     rdfs:comment "Used to link the derived concept of a bdqffdq:Validation to the bdqffdq:FundamentalConcept of a bdqffdq:Criterion."@en ;
                     rdfs:label "has Criterion"@en ;
                     skos:definition "The bdqffdq:Criterion under which a bdqffdq:Validation or bdqffdq:Issue assesses for data quality."@en ;
                     skos:prefLabel "has Criterion"@en .


###  https://rs.tdwg.org/bdqffdq/terms/hasDataQualityDimension
bdqffdq:hasDataQualityDimension rdf:type owl:ObjectProperty ;
                                rdfs:subPropertyOf bdqffdq:amendmentProperty ,
                                                   bdqffdq:issueProperty ,
                                                   bdqffdq:measurementProperty ,
                                                   bdqffdq:validationProperty ;
                                rdfs:range [ rdf:type owl:Restriction ;
                                             owl:onProperty bdqffdq:hasDataQualityDimension ;
                                             owl:someValuesFrom bdqffdq:DataQualityDimension
                                           ] ;
                                dcterms:issued "2024-09-30"^^xsd:date ;
                                rdfs:comment """Used to link a derived concept of a bdqffdq:DataQualityNeed (a Test, whether rdf:type Validation, Issue, Measure, or Amendment) to the bdqffdq:FundamentalConcept of a bdqffdq:DataQualityDimension. For a bdqffdq:Validation or bdqffdq:Issue, the bdqffdq:Dimension of data quality assessed. For a bdqffdq:Measure, the bdqffdq:Dimension of data quality measured. For a bdqffdq:Amendment, the bdqffdq:Dimension of data quality to be improved.

Under the original formulation of the Framework, only Measures have Dimensions."""@en ;
                                rdfs:label "has Data Quality Dimension"@en ;
                                skos:definition "The bdqffdq:DataQualityDimension to which a bdqffdq:DataQualityNeed applies."@en ;
                                skos:prefLabel "has Data Quality Dimension"@en .


###  https://rs.tdwg.org/bdqffdq/terms/hasEnhancement
bdqffdq:hasEnhancement rdf:type owl:ObjectProperty ;
                       rdfs:subPropertyOf bdqffdq:amendmentProperty ;
                       rdfs:range [ rdf:type owl:Restriction ;
                                    owl:onProperty bdqffdq:hasEnhancement ;
                                    owl:someValuesFrom bdqffdq:Enhancement
                                  ] ;
                       dcterms:issued "2024-09-30"^^xsd:date ;
                       rdfs:comment "Used to link the derived property of a bdqffdq:Amendment to the bdqffdq:FundamentalConcept of a bdqffdq:Enhancement."@en ;
                       rdfs:label "has Enhancement"@en ;
                       skos:definition "The bdqffdq:Enhancement that describes how a bdqffdq:Amendment may propose changes to improve data quality."@en ;
                       skos:prefLabel "has Enhancement"@en .


###  https://rs.tdwg.org/bdqffdq/terms/hasInformationElement
bdqffdq:hasInformationElement rdf:type owl:ObjectProperty ;
                              rdfs:subPropertyOf bdqffdq:amendmentProperty ,
                                                 bdqffdq:issueProperty ,
                                                 bdqffdq:measurementProperty ,
                                                 bdqffdq:validationProperty ;
                              rdfs:range bdqffdq:InformationElement ;
                              dcterms:issued "2024-09-30"^^xsd:date ;
                              rdfs:comment """Provides a relationship between bdqffdq:DataQualityNeed concepts and bdqffdq:InformationElements. For example, bdqffdq:Validation uses this property with bdqffdq:hasResourceType to define a bdqffdq:Criterion in the context of related bdqffdq:InformationElements.

Subtypes bdqffdq:hasActedUponInformationElement and bdqffdq:hasConsultedInformationElement allow a bdqffdq:DataQualityNeed to be related to specific bdqffdq:InformationElement terms in a way that allows bdqffdq:DataQualityReports to distinguish for consumers which bdqffdq:InformationElements a Test makes bdqffdq:Assertions about (and which only informed that bdqffdq:Assertion)."""@en ;
                              rdfs:label "has Information Element"@en ;
                              skos:definition "Describes the bdqffdq:InformationElements assessed by a bdqffdq:DataQualityNeed."@en ;
                              skos:prefLabel "has Information Element"@en .


###  https://rs.tdwg.org/bdqffdq/terms/hasParameter
bdqffdq:hasParameter rdf:type owl:ObjectProperty ;
                     rdfs:range bdqffdq:Parameter ;
                     dcterms:issued "2024-09-30"^^xsd:date ;
                     rdfs:comment "The bdqffdq:hasParameter property is expected to describe the Formal Parameter for which a bdqffdq:hasArgumentValue of the same bdqffdq:Argument provides the Actual Parameter. The bdqffdq:Argument is also expected to be the bdqffdq:hasArgument for a bdqffdq:Specification that provides the default value for the bdqffdq:hasArgumentValue and bdqffdq:hasParameter within a bdqffdq:hasAuthoritiesDefaults."@en ;
                     rdfs:label "has Parameter"@en ;
                     skos:definition "Relates a bdqffdq:Argument to a bdqffdq:Parameter."@en ;
                     skos:prefLabel "has Parameter"@en .


###  https://rs.tdwg.org/bdqffdq/terms/hasResourceType
bdqffdq:hasResourceType rdf:type owl:ObjectProperty ;
                        dcterms:issued "2024-09-30"^^xsd:date ;
                        rdfs:comment "Provides additional metadata, with the bdqffdq:InformationElements, that describe the bdqffdq:ResourceType (bdqffdq:SingleRecord or bdqffdq:MultiRecord) on which the bdqffdq: concept operates. For example, a bdqffdq:Amendment with bdqffdq:ResourceType bdqffdq:MultiRecord defines that bdqffdq:Amendment as operating on a data set."@en ;
                        rdfs:label "has Resource Type"@en ;
                        skos:definition "The bdqffdq:ResourceType to which a bdqffdq:DataQualityNeed applies."@en ;
                        skos:prefLabel "has Resource Type"@en .


###  https://rs.tdwg.org/bdqffdq/terms/hasResponseQualifier
bdqffdq:hasResponseQualifier rdf:type owl:ObjectProperty ;
                             rdfs:subPropertyOf bdqffdq:reportProperty ;
                             dcterms:issued "2024-09-30"^^xsd:date ;
                             rdfs:comment "Optional extension point, could be used to add structured information about uncertainty."@en ;
                             rdfs:label "has Response Qualifier"@en ;
                             skos:definition "ResponseQualifier object asserted by an Assertion."@en ;
                             skos:prefLabel "has Response Qualifier"@en .


###  https://rs.tdwg.org/bdqffdq/terms/hasResponseResult
bdqffdq:hasResponseResult rdf:type owl:ObjectProperty ;
                          rdfs:subPropertyOf bdqffdq:reportProperty ;
                          dcterms:issued "2024-09-30"^^xsd:date ;
                          rdfs:comment """Used in a bdqffdq:DataQualityReport to describe bdqffdq:ResponseResult objects. For example, values could be bdqffdq:COMPLIANT or bdqffdq:NOT_COMPLIANT for bdqffdq:ValidationAssertions. Both bdqffdq:ValidationAssertions and bdqffdq:IssueAssertions have bdqffdq:ResponseResults as objects. The bdqffdq:AmendmentAssertions have bdqffdq:ResponseResults that are data properties, so they are not expected to use this object property. The bdqffdq:MeasurementAssertion bdqffdq:ResponseResults may be objects or data.

If bdqffdq:ResponseResults are not objects, use the datatype property bdqffdq:hasResponseResultValue."""@en ;
                          rdfs:label "has Response Result"@en ;
                          skos:definition "The bdqffdq:ResponseResult object asserted by a bdqffdq:Assertion."@en ;
                          skos:prefLabel "has Response Result"@en .


###  https://rs.tdwg.org/bdqffdq/terms/hasResponseStatus
bdqffdq:hasResponseStatus rdf:type owl:ObjectProperty ;
                          rdfs:subPropertyOf bdqffdq:reportProperty ;
                          dcterms:issued "2024-09-30"^^xsd:date ;
                          rdfs:comment """Used in a bdqffdq:DataQualityReport to describe bdqffdq:ResponseStatus. For example, in the case of a bdqffdq:ValidationAssertion, bdqffdq:ResponseStatus values could be bdqffdq:RUN_HAS_RESULT, bdqffdq:INTERNAL_PREREQUISITES_NOT_MET, or bdqffdq:EXTERNAL_PREREQISITES_NOT_MET. Similarly, bdqffdq:AmendmentAssertions can assert bdqffdq:ResponesStatus objects including bdqffdq:AMENDED or bdqffdq:FILLED_IN.

The bdqffdq:ResponseStatus is always an object, unlike bdqffdq:ResponseResult, where either the object property bdqffdq:hasResponseResult or the data property bdqffdq:hasResponseResultValue may apply."""@en ;
                          rdfs:label "has Response Status"@en ;
                          skos:definition "The bdqffdq:ResponseStatus object asserted by a bdqffdq:Assertion."@en ;
                          skos:prefLabel "has Response Status"@en .


###  https://rs.tdwg.org/bdqffdq/terms/hasSpecification
bdqffdq:hasSpecification rdf:type owl:ObjectProperty ;
                         rdfs:range [ rdf:type owl:Restriction ;
                                      owl:onProperty bdqffdq:hasSpecification ;
                                      owl:someValuesFrom bdqffdq:Specification
                                    ] ;
                         dcterms:issued "2024-09-30"^^xsd:date ;
                         rdfs:comment "Describes the relationship between a derived bdqffdq: concept that is a bdqffdq:Method and the bdqffdq:FundamentalConcept of a bdqffdq:Specification (technical description of a Test)."@en ;
                         rdfs:label "has Specification"@en ;
                         skos:definition "Relates a bdqffdq:Method to a bdqffdq:Specification."@en ;
                         skos:prefLabel "has Specification"@en .


###  https://rs.tdwg.org/bdqffdq/terms/hasUseCase
bdqffdq:hasUseCase rdf:type owl:ObjectProperty ;
                   rdfs:range [ rdf:type owl:Restriction ;
                                owl:onProperty bdqffdq:hasUseCase ;
                                owl:someValuesFrom bdqffdq:UseCase
                              ] ;
                   dcterms:issued "2024-09-30"^^xsd:date ;
                   rdfs:comment "Used by concepts in the bdqffdq:DataQualityNeed category to describe the relationship between bdqffdq:Policies (bdqffdq:ValidationPolicy, bdqffdq:MeasurementPolicy, bdqffdq:AmendmentPolicy) and an instance of a bdqffdq:UseCase."@en ;
                   rdfs:label "has Use Case"@en ;
                   skos:definition "Relates a bdqffdq:Policy to a bdqffdq:UseCase."@en ;
                   skos:prefLabel "has Use Case"@en .


###  https://rs.tdwg.org/bdqffdq/terms/implementedBy
bdqffdq:implementedBy rdf:type owl:ObjectProperty ;
                      rdfs:range [ rdf:type owl:Restriction ;
                                   owl:onProperty bdqffdq:implementedBy ;
                                   owl:someValuesFrom bdqffdq:Mechanism
                                 ] ;
                      dcterms:issued "2024-09-30"^^xsd:date ;
                      rdfs:comment "Describes the link between a bdqffdq:Implementation and a bdqffdq:Mechanism."@en ;
                      rdfs:label "implemented By"@en ;
                      skos:definition "The bdqffdq:Mechanism that provides a bdqffdq:Implementation"@en ;
                      skos:prefLabel "implemented By"@en .


###  https://rs.tdwg.org/bdqffdq/terms/improvedBy
bdqffdq:improvedBy rdf:type owl:ObjectProperty ;
                   rdfs:range [ rdf:type owl:Restriction ;
                                owl:onProperty bdqffdq:improvedBy ;
                                owl:someValuesFrom bdqffdq:Amendment
                              ] ;
                   dcterms:issued "2024-09-30"^^xsd:date ;
                   rdfs:comment """Originally had Domain: Amendment and Range: ImprovementTarget. Asserts that a bdqffdq:ImprovementTarget could be improved by the bdqffdq:Amendment.

Object property that describes a bdqffdq:Amendment, as part of the bdqffdq:ImprovementTarget, that would improve data bdqffdq:ActedUpon by a set of bdqffdq:Measures or bdqffdq:Validations. This can be used to determine which bdqffdq:Measures and bdqffdq:Validations are improved upon by a given bdqffdq:Amendment."""@en ;
                   rdfs:label "improved By"@en ;
                   skos:definition "The bdqffdq:ImprovementTarget that would have data quality improved by bdqffdq:Assertions resulting from a bdqffdq:Amendment."@en ;
                   skos:prefLabel "improved By"@en .


###  https://rs.tdwg.org/bdqffdq/terms/includedInPolicy
bdqffdq:includedInPolicy rdf:type owl:ObjectProperty ;
                         dcterms:issued "2024-09-30"^^xsd:date ;
                         rdfs:comment "Relates bdqffdq:Policies to Tests (bdqffdq:DataQualityNeed)."@en ;
                         rdfs:label "included In Policy"@en ;
                         skos:definition "Assserts that a bdqffdq:DataQualityNeed is part of a bdqffdq:Policy."@en ;
                         skos:prefLabel "included In Policy"@en .


###  https://rs.tdwg.org/bdqffdq/terms/issueProperty
bdqffdq:issueProperty rdf:type owl:ObjectProperty ;
                      dcterms:issued "2024-09-30"^^xsd:date ;
                      rdfs:comment "Properties that relate bdqffdq:Issues to bdqffdq:IssueMethods, bdqffdq:Criteria, and bdqffdq:DataQualityDimensions."@en ;
                      rdfs:label "issue Property"@en ;
                      skos:definition "Category of object properties that apply to bdqffdq:Issues."@en ;
                      skos:prefLabel "issue Property"@en .


###  https://rs.tdwg.org/bdqffdq/terms/measurementProperty
bdqffdq:measurementProperty rdf:type owl:ObjectProperty ;
                            dcterms:issued "2024-09-30"^^xsd:date ;
                            rdfs:comment "Subproperties of this type group object properties that apply to bdqffdq:MeasurementConcepts such as bdqffdq:MeasurementPolicy (bdqffdq:DataQualityNeed), bdqffdq:MeasurementMethod (bdqffdq:DataQualityMethod) and bdqffdq:Measure (bdqffdq:DataQualityReport)."@en ;
                            rdfs:label "measurement Property"@en ;
                            skos:definition "Category of object properties that apply to bdqffdq:Measures."@en ;
                            skos:prefLabel "measurement Property"@en .


###  https://rs.tdwg.org/bdqffdq/terms/producesAssertion
bdqffdq:producesAssertion rdf:type owl:ObjectProperty ;
                          dcterms:issued "2024-09-30"^^xsd:date ;
                          rdfs:comment "Connects bdqffdq:Implementations (Solutions layer, see Figure 3 in Veiga et al., 2017) with the bdqffdq:Assertions (Reports layer, see Figure 3 in Veiga et al., 2017) that they produce from the execution of a bdqffdq:Specification."@en ;
                          rdfs:label "produces Assertion"@en ;
                          skos:definition "Connects an entity with a bdqffdq:Assertion that the entity created."@en ;
                          skos:prefLabel "produces Assertion"@en .


###  https://rs.tdwg.org/bdqffdq/terms/reportProperty
bdqffdq:reportProperty rdf:type owl:ObjectProperty ;
                       dcterms:issued "2024-09-30"^^xsd:date ;
                       rdfs:comment "Category of properties used in reports (object properties associated with response objects (bdqffdq:Assertions)). See also the data properties bdqffdq:hasResponseComment and bdqffdq:hasResponseResultValue."@en ;
                       rdfs:label "report Property"@en ;
                       skos:definition "Category of object properties that apply to bdqffdq:Assertions."@en ;
                       skos:prefLabel "report Property"@en .


###  https://rs.tdwg.org/bdqffdq/terms/targetedIssue
bdqffdq:targetedIssue rdf:type owl:ObjectProperty ;
                      rdfs:range [ rdf:type owl:Restriction ;
                                   owl:onProperty bdqffdq:targetedIssue ;
                                   owl:someValuesFrom bdqffdq:Issue
                                 ] ;
                      dcterms:issued "2024-09-30"^^xsd:date ;
                      rdfs:comment "The bdqffdq:Issue targeted by a problem via the bdqffdq:ImprovementTarget object. Describes the relationship between a bdqffdq:ImprovementTarget and a bdqffdq:Issue."@en ;
                      rdfs:label "targeted Issue"@en ;
                      skos:definition "A bdqffdq:Issue for which the data conformance with a bdqffdq:NeedConcept may be improved by accepting proposals from a bdqffdq:Amendment via a bdqffdq:ImprovementTarget."@en ;
                      skos:prefLabel "targeted Issue"@en .


###  https://rs.tdwg.org/bdqffdq/terms/targetedMeasure
bdqffdq:targetedMeasure rdf:type owl:ObjectProperty ;
                        rdfs:range [ rdf:type owl:Restriction ;
                                     owl:onProperty bdqffdq:targetedMeasure ;
                                     owl:someValuesFrom bdqffdq:Measure
                                   ] ;
                        dcterms:issued "2024-09-30"^^xsd:date ;
                        rdfs:comment "Describes the relationship between a bdqffdq:ImprovementTarget and a bdqffdq:Measure."@en ;
                        rdfs:label "targeted Measure"@en ;
                        skos:definition "A bdqffdq:Measure for which the data conformance with a bdqffdq:NeedConcept may be improved by accepting proposals from a bdqffdq:Amendment via a bdqffdq:ImprovementTarget."@en ;
                        skos:prefLabel "targeted Measure"@en .


###  https://rs.tdwg.org/bdqffdq/terms/targetedValidation
bdqffdq:targetedValidation rdf:type owl:ObjectProperty ;
                           rdfs:subPropertyOf owl:topObjectProperty ;
                           rdfs:range [ rdf:type owl:Restriction ;
                                        owl:onProperty bdqffdq:targetedValidation ;
                                        owl:someValuesFrom bdqffdq:Validation
                                      ] ;
                           dcterms:issued "2024-09-30"^^xsd:date ;
                           rdfs:comment "Relates a bdqffdq:ImprovementTarget to a bdqffdq:Validation. Describes the relationship between a bdqffdq:ImprovementTarget and a bdqffdq:Validation."@en ;
                           rdfs:label "targeted Validation"@en ;
                           skos:definition "A bdqffdq:Validation for which the data conformance with a bdqffdq:NeedConcept may be improved by accepting proposals from a bdqffdq:Amendment via a bdqffdq:ImprovementTarget."@en ;
                           skos:prefLabel "targeted Validation"@en .


###  https://rs.tdwg.org/bdqffdq/terms/usesSpecification
bdqffdq:usesSpecification rdf:type owl:ObjectProperty ;
                          rdfs:range [ rdf:type owl:Restriction ;
                                       owl:onProperty bdqffdq:usesSpecification ;
                                       owl:someValuesFrom bdqffdq:Specification
                                     ] ;
                          dcterms:issued "2024-09-30"^^xsd:date ;
                          rdfs:comment "Relates a bdqffdq:Implementation to the bdqffdq:Specification that the bdqffdq:Implementation implements."@en ;
                          rdfs:label "uses Specification"@en ;
                          skos:definition "The bdqffdq:Specification that a bdqffdq:Implementation implements."@en ;
                          skos:prefLabel "uses Specification"@en .


###  https://rs.tdwg.org/bdqffdq/terms/validationProperty
bdqffdq:validationProperty rdf:type owl:ObjectProperty ;
                           dcterms:issued "2024-09-30"^^xsd:date ;
                           rdfs:comment "Subproperties of this type group object properties that apply to bdqffdq:ValidationConcepts such as bdqffdq:ValidationPolicy (bdqffdq:DataQualityNeed), bdqffdq:ValidationMethod (bdqffdq:DataQualityMethod) and bdqffdq:Validation (bdqffdq:DataQualityReport)."@en ;
                           rdfs:label "validation Property"@en ;
                           skos:definition "Category of object properties that apply to bdqffdq:Validations."@en ;
                           skos:prefLabel "validation Property"@en .


#################################################################
#    Data properties
#################################################################

###  https://rs.tdwg.org/bdqffdq/terms/hasArgumentValue
bdqffdq:hasArgumentValue rdf:type owl:DatatypeProperty ;
                         dcterms:issued "2024-09-30"^^xsd:date ;
                         rdfs:label "has Argument Value"@en ;
                         skos:definition "The value of a bdqffdq:Argument that is used in a bdqffdq:Specification to replace a Formal Parameter to determine the behavior of the bdqffdq:Specification."@en ;
                         skos:prefLabel "has Argument value"@en .


###  https://rs.tdwg.org/bdqffdq/terms/hasAuthoritiesDefaults
bdqffdq:hasAuthoritiesDefaults rdf:type owl:DatatypeProperty ;
                               rdfs:range xsd:string ;
                               dcterms:issued "2024-09-30"^^xsd:date ;
                               rdfs:comment "Details of the bdq:sourceAuthority listed in a bdqffdq:Specification, with bdqffdq:Parameters that may affect the bdqffdq:hasExpectedResponse, and with their default values."@en ;
                               rdfs:label "has Authorities and Defaults"@en ;
                               skos:definition "Text describing bdq:sourceAuthorities and bdqffdq:Parameters with their default values to attach to a bdqffdq:Specification to further specify the behavior described in the bdqffdq:hasExpectedResponse."@en ;
                               skos:prefLabel "has Authorities and Defaults"@en .


###  https://rs.tdwg.org/bdqffdq/terms/hasDateLastUpdated
bdqffdq:hasDateLastUpdated rdf:type owl:DatatypeProperty ;
                           rdfs:subPropertyOf owl:topDataProperty ;
                           rdfs:range xsd:date ;
                           dcterms:issued "2024-09-30"^^xsd:date ;
                           rdfs:comment "While a new instance of a resource with a new dcterms:issued is required for any change to that resource, not all changes would be pertinent to implementers, (i.e., that would required implementers to evaluate their code for changes needed to comply with the update). The bdqffdq:hasDateLastUpdated allows implementers to identify which new changes to the definition of a Test would entail changes to code, and which would not. For example, a change to the logic of a bdqffdq:Specification in the text of bdqffdq:hasExpectedResponse would imply needed changes to the logic of code implementing that bdqffdq:Specification, but a correction of a spelling mistake within the text of a bdqffdq:hasExpectedResponse would not."@en ;
                           rdfs:label "has Date Last Updated"@en ;
                           skos:definition "Date of the most recent dcterms:issued for this class with a change that would be pertinent to a bdqffdq:Implementation."@en ;
                           skos:prefLabel "has Date Last Updated"@en .


###  https://rs.tdwg.org/bdqffdq/terms/hasExpectedResponse
bdqffdq:hasExpectedResponse rdf:type owl:DatatypeProperty ;
                            rdfs:range xsd:string ;
                            dcterms:issued "2024-09-30"^^xsd:date ;
                            rdfs:comment "The description of the logic of a Test Specification. A bdqffdq:hasExpectedResponse is expected to be a data property of a Specification."@en ;
                            rdfs:label "has Expected Response"@en ;
                            skos:definition "Text describing the logic to be followed by a bdqffdq:Implementation of a bdqffdq:Specification specifying the values of bdqffdq:ResponseStatus and bdqffdq:ResponseResults that should be produced from the evaluation of input bdqffdq:InformationElements."@en ;
                            skos:prefLabel "has Expected Response"@en .


###  https://rs.tdwg.org/bdqffdq/terms/hasResponseComment
bdqffdq:hasResponseComment rdf:type owl:DatatypeProperty ;
                           rdfs:range xsd:string ;
                           dcterms:issued "2024-09-30"^^xsd:date ;
                           rdfs:comment "Intended for consumption by human readers of bdqffdq:DataQualityReports to understand why particular bdqffdq:Assertions were made."@en ;
                           rdfs:label "has Response Comment"@en ;
                           skos:definition "Free text describing the bdqffdq:Assertion made in the response and why that conclusion was reached."@en ;
                           skos:prefLabel "has Response Comment"@en .


###  https://rs.tdwg.org/bdqffdq/terms/hasResponseResultValue
bdqffdq:hasResponseResultValue rdf:type owl:DatatypeProperty ;
                               dcterms:issued "2024-09-30"^^xsd:date ;
                               rdfs:comment "Applies to bdqffdq:AmendmentAssertions. To support bdqtest: Tests, bdqffdq:hasResponseResultValue is expected to carry a key:value list where the keys are the names of bdqffdq:ActedUpon bdqffdq:InformationElements, and the values are the proposed new values (filling in or replacing the values of those terms in the input). Applies to bdqffdq:MeasureAssertions that assert a numeric value."@en ;
                               rdfs:label "has response result value"@en ;
                               skos:definition "Data property carrying the value of a bdqffdq:Assertion when the value is not an object."@en ;
                               skos:prefLabel "has response result value"@en .


#################################################################
#    Classes
#################################################################

###  https://rs.tdwg.org/bdqffdq/terms/AbstractInformationElement
bdqffdq:AbstractInformationElement rdf:type owl:Class ;
                                   rdfs:subClassOf bdqffdq:InformationElement ;
                                   dcterms:issued "2024-09-30"^^xsd:date ;
                                   rdfs:comment "Such bdqffdq:InformationElements as DATE and DAY are abstract, they could reference any representation of those concepts. In contrast, dwc:eventDate and dwc:day can be linked to concrete bdqffdq:ActedUponInformationElements or bdqffdq:ConsultedInformationElements."@en ;
                                   rdfs:label "Abstract Information Element"@en ;
                                   skos:definition "A bdqffdq:InformationElement described in abstract terms and not linked with any concrete terms."@en ;
                                   skos:prefLabel "Abstract Information Element"@en .


###  https://rs.tdwg.org/bdqffdq/terms/ActedUpon
bdqffdq:ActedUpon rdf:type owl:Class ;
                  rdfs:subClassOf bdqffdq:InformationElement ;
                  dcterms:issued "2024-09-30"^^xsd:date ;
                  rdfs:comment "A bdqffdq:InformationElement to which a bdqffdq:ResponseResult applies."@en ;
                  rdfs:label "Acted Upon"@en ;
                  skos:definition "A bdqffdq:InformationElement, expressed in concrete terms, about which a bdqffdq:DataQualityNeed expresses bdqffdq:Assertions about the data quality in that bdqffdq:InformationElement."@en ;
                  skos:prefLabel "Acted Upon"@en .


###  https://rs.tdwg.org/bdqffdq/terms/Amendment
bdqffdq:Amendment rdf:type owl:Class ;
                  rdfs:subClassOf bdqffdq:AmendmentConcept ,
                                  bdqffdq:DataQualityNeed ;
                  dcterms:issued "2024-09-30"^^xsd:date ;
                  rdfs:comment """ContextualizedEnhacement in the original framework. Describes an instance of a bdqffdq:Enhancement in the context of the associated bdqffdq:InformationElements from a controlled vocabulary (fields bdqffdq:ActedUpon or bdqffdq:Consulted), and a bdqffdq:ResourceType of bdqffdq:SingleRecord or bdqffdq:MultiRecord.

Describes a proposal for a bdqffdq:Enhancement of original data, which if accepted, would improve the quality of the data for a use. For example: 'Recommends valid value for taxon name in a Single Record.'

bdqffdq:Amendments may describe proposed changes to data values, or proposed changes to processes for the production and manipulation of data, for example, a bdqffdq:Amendment on a bdqffdq:SingleRecord may provide bdqffdq:Criteria for proposing that dwc:decimalLatitude and dwc:decimalLongitude are transposed in that record. Similarly, a bdqffdq:Amendment on a bdqffdq:MultiRecord may provide bdqffdq:Critera for proposing that all dwc:decimalLatitudes and dwc:decimalLongitudes from a data source have been transposed, and the mapping of data values to transport terms should be changed.

A bdqffdq:Amendment is the bdqffdq:DataQualityNeed that parallels a bdqffdq:AmendmentMethod in the Solutions layer (see Figure 3 in Veiga et al., 2017), and a bdqffdq:AmendmentAssertion in the Report layer (see Figure 3 in Veiga et al., 2017).

AM = { am | am = < ie, e, rt >, ie ∈ IE, e ∈ E ⋀ rt ∈ RT }"""@en ;
                  rdfs:label "Amendment"@en ;
                  skos:definition "A bdqffdq:DataQualityNeed that expresses how proposals may be made to improve the fitness for use of data."@en ;
                  skos:prefLabel "Amendment"@en .


###  https://rs.tdwg.org/bdqffdq/terms/AmendmentAssertion
bdqffdq:AmendmentAssertion rdf:type owl:Class ;
                           rdfs:subClassOf bdqffdq:AmendmentConcept ,
                                           bdqffdq:Assertion ;
                           dcterms:issued "2024-09-30"^^xsd:date ;
                           rdfs:comment """The bdqffdq:AmendmentAssertion type is a Report layer concept (see Figure 3 in Veiga et al., 2017) that describes the results of the execution of a Test that performs a bdqffdq:AmendmentMethod following a bdqffdq:Specification to propose changes based on a bdqffdq:Amendment. 

A bdqffdq:Amendment is expected to carry a bdqffdq:ResponseStatus result that includes a status bdqffdq:FILLED_IN or bdqffdq:AMENDED, as well as a bdqffdq:ResponseResult that asserts proposed changes to values from the original data.

DQA(dr) = {dqa | dqa = < am, s, m, r >, am ∈ AM, s ∈ S, m ∈ M , r ∈ R ⋀ dr ∈ DR}"""@en ;
                           rdfs:label "Amendment Assertion"@en ;
                           skos:definition "A bdqffdq:Assertion expressing the result of a bdqffdq:Implementation evaluating a bdqffdq:Amendment supporting a particular bdqffdq:DataQualityNeed to improve a particular bdqffdq:DataResource."@en ;
                           skos:prefLabel "Amendment Assertion"@en .


###  https://rs.tdwg.org/bdqffdq/terms/AmendmentConcept
bdqffdq:AmendmentConcept rdf:type owl:Class ;
                         dcterms:issued "2024-09-30"^^xsd:date ;
                         rdfs:label "Amendment Concept"@en ;
                         skos:definition "A term involved in proposals of changes to data or process to improve data quality to fit an expressed bdqffdq:DataQualityNeed."@en ;
                         skos:prefLabel "Amendment Concept"@en .


###  https://rs.tdwg.org/bdqffdq/terms/AmendmentMethod
bdqffdq:AmendmentMethod rdf:type owl:Class ;
                        rdfs:subClassOf bdqffdq:AmendmentConcept ,
                                        bdqffdq:DataQualityMethod ;
                        dcterms:issued "2024-09-30"^^xsd:date ;
                        rdfs:comment """The bdqffdq:AmendmentMethod is a bdqffdq:DataQualityMethod describing the relationship between a bdqffdq:Specification (technical description of a Test) and a bdqffdq:Amendment (a bdqffdq:Enhancement in the context of bdqffdq:ResourceType (bdqffdq:SingleRecord or bdqffdq:MultiRecord) and associated bdqffdq:InformationElements).

EM(am) = {s | s ⊂ S ⋀ am ∈ AM}"""@en ;
                        rdfs:label "Amendment Method"@en ;
                        skos:definition "A data quality bdqffdq:SolutionsConcept that relates a bdqffdq:Amendment to its bdqffdq:Specifications."@en ;
                        skos:prefLabel "Amendment Method"@en .


###  https://rs.tdwg.org/bdqffdq/terms/AmendmentPolicy
bdqffdq:AmendmentPolicy rdf:type owl:Class ;
                        rdfs:subClassOf bdqffdq:AmendmentConcept ,
                                        bdqffdq:Policy ;
                        dcterms:issued "2024-09-30"^^xsd:date ;
                        rdfs:comment """A data quality Need layer concept (see Figure 3 in Veiga et al., 2017) that describes how a bdqffdq:Amendment relates to a bdqffdq:UseCase. This relationship defines which bdqffdq:Amendments are supported by a given bdqffdq:UseCase.

EP(u) = {am | am ⊂ AM ⋀ u ∈ U }"""@en ;
                        rdfs:label "Amendment Policy"@en ;
                        skos:definition "A bdqffdq:NeedConcept that relates a bdqffdq:UseCase to a set of supporting bdqffdq:Amendments."@en ;
                        skos:prefLabel "Amendment Policy"@en .


###  https://rs.tdwg.org/bdqffdq/terms/Argument
bdqffdq:Argument rdf:type owl:Class ;
                 rdfs:subClassOf bdqffdq:SolutionsConcept ;
                 dcterms:issued "2024-09-30"^^xsd:date ;
                 rdfs:comment "The bdqffdq:Argument is an Actual Parameter, for which a bdqffdq:Parameter is the corresponding Formal Parameter. An extension to the original fitness for use framework as described in Veiga et al., 2017."@en ;
                 rdfs:label "Argument"@en ;
                 skos:definition "A value that, when provided to a Test bdqffdq:Specification to replace a bdqffdq:Parameter changes the behavior of the Test in a defined manner."@en ;
                 skos:prefLabel "Argument"@en .


###  https://rs.tdwg.org/bdqffdq/terms/Assertion
bdqffdq:Assertion rdf:type owl:Class ;
                  rdfs:subClassOf bdqffdq:ReportConcept ;
                  dcterms:issued "2024-09-30"^^xsd:date ;
                  rdfs:comment "The bdqffdq:Assertion type is the bdqffdq:FundamentalConcept that makes up a bdqffdq:DataQualityReport. A bdqffdq:Assertion can be any one of four types (represented as subclasses), bdqffdq:Validation, bdqffdq:Issue, bdqffdq:Measure, and bdqffdq:Amendment. The bdqffdq:Assertion concept consists of a bdqffdq:Specification (the technical description of a performed Test), a bdqffdq:DataResource (initial values of input data expressed in terms of a controlled vocabulary), the bdqffdq:Mechanism (external service, actor, or code that performs the Test), and a form of result."@en ;
                  rdfs:label "Assertion"@en ;
                  skos:definition "A bdqffdq:ReportConcept expressing a statement about a data quality bdqffdq:Assertion following a bdqffdq:Specification produced by a bdqffdq:Implementation pertaining to a bdqffdq:DataResource."@en ;
                  skos:prefLabel "Assertion"@en .


###  https://rs.tdwg.org/bdqffdq/terms/Consulted
bdqffdq:Consulted rdf:type owl:Class ;
                  rdfs:subClassOf bdqffdq:InformationElement ;
                  dcterms:issued "2024-09-30"^^xsd:date ;
                  rdfs:comment "A bdqffdq:InformationElement the content of which is examined to assert a result on one or more other bdqffdq:InformationElements."@en ;
                  rdfs:label "Consulted"@en ;
                  skos:definition "A bdqffdq:InformationElement, expressed in concrete terms, about which a bdqffdq:DataQualityNeed examines in order to expresses bdqffdq:Assertions about the data quality in another bdqffdq:InformationElement."@en ;
                  skos:prefLabel "Acted Upon"@en .


###  https://rs.tdwg.org/bdqffdq/terms/Criterion
bdqffdq:Criterion rdf:type owl:Class ;
                  rdfs:subClassOf bdqffdq:FundamentalConcept ,
                                  bdqffdq:NeedConcept ;
                  dcterms:issued "2024-09-30"^^xsd:date ;
                  rdfs:comment "General statement, for example, 'In a controlled vocabulary.' Composed with both bdqffdq:Validations and bdqffdq:Issues."@en ;
                  rdfs:label "Criterion"@en ;
                  skos:definition "Rule against which data are evaluated for conformance to quality bdqffdq:Criteria."@en ;
                  skos:prefLabel "Criterion"@en .


###  https://rs.tdwg.org/bdqffdq/terms/DataQualityDimension
bdqffdq:DataQualityDimension rdf:type owl:Class ;
                             rdfs:subClassOf bdqffdq:FundamentalConcept ,
                                             bdqffdq:NeedConcept ;
                             dcterms:issued "2024-09-30"^^xsd:date ;
                             rdfs:comment "Describes the aspect of data quality (accuracy, precision, completeness, etc.) that a Test examines. For example, [precision] in [coordinate precision of Single Records]. In the original framework, only related to Measures, here may be related to any bdqffdq:DataQualityNeed."@en ;
                             rdfs:label "Data Quality Dimension"@en ;
                             skos:definition "An aspect of data quality."@en ;
                             skos:prefLabel "Data Quality Dimension"@en .


###  https://rs.tdwg.org/bdqffdq/terms/DataQualityMethod
bdqffdq:DataQualityMethod rdf:type owl:Class ;
                          rdfs:subClassOf bdqffdq:SolutionsConcept ;
                          dcterms:issued "2024-09-30"^^xsd:date ;
                          rdfs:comment "A bdqffdq:DataQualityMethod is an associative entity that allows bdqffdq:Specifications or data quality Tests to be reused by supporting a many-to-many relationship between the two."@en ;
                          rdfs:label "Data Quality Method"@en ;
                          skos:definition "A bdqffdq:SolutionsConcept that relates a bdqffdq:DataQualityNeed to a bdqffdq:Specification."@en ;
                          skos:prefLabel "Data Quality Method"@en .


###  https://rs.tdwg.org/bdqffdq/terms/DataQualityNeed
bdqffdq:DataQualityNeed rdf:type owl:Class ;
                        rdfs:subClassOf bdqffdq:NeedConcept ;
                        dcterms:issued "2024-09-30"^^xsd:date ;
                        rdfs:comment "Subtypes of bdqffdq:DataQualityNeed are the Test Types (Validation, Issue, Measure, and Amendment). The bdqffdq:DataQualityNeed appoximates the informal concept of a Test as used in the BDQ standard."@en ;
                        rdfs:label "Data Quality Need"@en ;
                        skos:definition "A bdqffdq:NeedConcept that expresses what bdqffdq:Assertions may be made about data with respect to fitness for use."@en ;
                        skos:prefLabel "Data Quality Need"@en .


###  https://rs.tdwg.org/bdqffdq/terms/DataQualityProfile
bdqffdq:DataQualityProfile rdf:type owl:Class ;
                           rdfs:subClassOf bdqffdq:NeedConcept ;
                           dcterms:issued "2024-09-30"^^xsd:date ;
                           rdfs:comment """The bdqffdq:DataQualityProfile is a data quality Need layer concept (see Figure 3 in Veiga et al., 2017) describing the bdqffdq:UseCases that make up a data quality operation such as the behavior of a single actor or workflow producing the relevant bdqffdq:Assertions.

DQP (u) = {dqp | dqp = mp(u) ⋃ vp(u) ⋃ ep(u), mp ∈ MP , vp ∈ VP , ep ∈ EP ⋀ u ∈ U }"""@en ;
                           rdfs:label "Data Quality Profile"@en ;
                           skos:definition "A bdqffdq:NeedConcept expressing the composition of bdqffdq:Policies to satisfy a bdqffdq:UseCase."@en ;
                           skos:prefLabel "Data Quality Profile"@en .


###  https://rs.tdwg.org/bdqffdq/terms/DataQualityReport
bdqffdq:DataQualityReport rdf:type owl:Class ;
                          rdfs:subClassOf bdqffdq:ReportConcept ;
                          dcterms:issued "2024-09-30"^^xsd:date ;
                          rdfs:comment "A bdqffdq:DataQualityReport consists of a set of bdqffdq:Assertions (bdqffdq:ValidationAssertions, bdqffdq:IssueAssertions, bdqffdq:MeasureAssertions, and bdqffdq:AmendmentAssertions) that represent the output of a workflow/actor run. These bdqffdq:Assertions form an account of the fitness for use of a tested data set for a specified bdqffdq:UseCase, as produced by a bdqffdq:Mechanism."@en ;
                          rdfs:label "Data Quality Report"@en ;
                          skos:definition "A bdqffdq:ReportConcept comprising a set of data quality bdqffdq:Assertions."@en ;
                          skos:prefLabel "Data Quality Report"@en .


###  https://rs.tdwg.org/bdqffdq/terms/DataResource
bdqffdq:DataResource rdf:type owl:Class ;
                     rdfs:subClassOf bdqffdq:ReportConcept ;
                     dcterms:issued "2024-09-30"^^xsd:date ;
                     rdfs:comment """Describes a bdqffdq:DataResource containing terms from a vocabulary such as Darwin Core that can be related to bdqffdq:InformationElements, and represents the original values of the data operated on by a bdqffdq:Assertion Test (e.g., an instance of dwc:Occurrence). Ideally, bdqffdq:DataResources have persistent GUIDs.

A bdqffdq:DataResource could be the oa:target of a oa:Annotation of which a bdqffdq:Assertion is the oa:body.

DR = { dr | dr = < id, rt, v >, id ∈ I D, rt ∈ RT , (rt = sr ⋁ rt = ds) ⋀ v ∈ V }"""@en ;
                     rdfs:label "Data Resource"@en ;
                     skos:definition "An owl:Thing to which a data quality bdqffdq:Assertion applies."@en ;
                     skos:prefLabel "Data Resource"@en .


###  https://rs.tdwg.org/bdqffdq/terms/Enhancement
bdqffdq:Enhancement rdf:type owl:Class ;
                    rdfs:subClassOf bdqffdq:AmendmentConcept ,
                                    bdqffdq:FundamentalConcept ,
                                    bdqffdq:NeedConcept ;
                    dcterms:issued "2024-09-30"^^xsd:date ;
                    rdfs:comment "A general statement about improvement, for example, 'Recommend replacement value from a controlled vocabulary'."@en ;
                    rdfs:label "Enhancement"@en ;
                    skos:definition "Description of a means by which data could be improved."@en ;
                    skos:prefLabel "Enhancement"@en .


###  https://rs.tdwg.org/bdqffdq/terms/FundamentalConcept
bdqffdq:FundamentalConcept rdf:type owl:Class ;
                           dcterms:issued "2024-09-30"^^xsd:date ;
                           rdfs:comment "Contrast with derived concepts, which are compositions of two or more bdqffdq:FundamentalConcepts, see Veiga et al., 2017. Derived concepts can be organized by Test type into bdqffdq:ValidationConcept, bdqffdq:IssueConcept, bdqffdq:MeasurementConcept, or bdqffdq:AmendmentConcept. Derived concepts can also be organized by framework layer into bdqffdq:NeedConcept, bdqffdq:SolutionsConcept, and bdqffdq:ReportConcept (see Figure 3 in Veiga et al., 2017)."@en ;
                           rdfs:label "Fundamental Concept"@en ;
                           skos:definition "Category of fitness for use concepts that are not derived by composition with other concepts."@en ;
                           skos:prefLabel "Fundamental Concept"@en .


###  https://rs.tdwg.org/bdqffdq/terms/Implementation
bdqffdq:Implementation rdf:type owl:Class ;
                       rdfs:subClassOf bdqffdq:SolutionsConcept ;
                       dcterms:issued "2024-09-30"^^xsd:date ;
                       rdfs:comment """A bdqffdq:Implementation describes the relationship between a bdqffdq:Specification (technical description of a Test) and the bdqffdq:Mechanism that implements it.

I (s) = {m | m ⊂ M ⋀ s ∈ S}"""@en ;
                       rdfs:label "Implementation"@en ;
                       skos:definition "A bdqffdq:SolutionsConcept that describes the portion of a bdqffdq:Mechanism that carries out the proccess described in a particular bdqffdq:Specification."@en ;
                       skos:prefLabel "Implementation"@en .


###  https://rs.tdwg.org/bdqffdq/terms/ImprovementTarget
bdqffdq:ImprovementTarget rdf:type owl:Class ;
                          rdfs:subClassOf bdqffdq:NeedConcept ;
                          dcterms:issued "2024-09-30"^^xsd:date ;
                          rdfs:comment """A bdqffdq:ImprovementTarget describes which bdqffdq:Validations, bdqffdq:Issues, and bdqffdq:Measures are improved by a bdqffdq:Amendment. The bdqffdq:ImprovementTarget includes relationships between a bdqffdq:Amendment and one or more bdqffdq:Validations or bdqffdq:Measures.

IT(am) = {me ⋃ va | me ∈ ME, va ∈ VA ⋀ am ∈ AM}"""@en ;
                          rdfs:label "Improvement Target"@en ;
                          skos:definition "A specific bdqffdq:DataQualityNeed that a specific bdqffdq:Amendment is intended to improve."@en ;
                          skos:prefLabel "Improvement Target"@en .


###  https://rs.tdwg.org/bdqffdq/terms/InformationElement
bdqffdq:InformationElement rdf:type owl:Class ;
                           rdfs:subClassOf bdqffdq:FundamentalConcept ;
                           dcterms:issued "2024-09-30"^^xsd:date ;
                           rdfs:comment "A bdqffdq:InformationElement identifies a portion of data to which a Test pertains. A bdqffdq:InformationElement can be represented as a single or composite element that consists of one or more terms from a controlled vocabulary (fields bdqffdq:ActedUpon or bdqffdq:Consulted by a bdqffdq:Assertion Test) that identifies concepts in data relevant to a bdqffdq:UseCase. An abstraction or a concrete term that represents relevant content (e.g., coordinates; dwc:decimalLatitude, dwc:decimalLongitude)."@en ;
                           rdfs:label "Information Element"@en ;
                           skos:definition "A portion of data with which a bdqffdq:DataQualityNeed is concerned."@en ;
                           skos:prefLabel "Information Element"@en .


###  https://rs.tdwg.org/bdqffdq/terms/Issue
bdqffdq:Issue rdf:type owl:Class ;
              rdfs:subClassOf bdqffdq:DataQualityNeed ,
                              bdqffdq:IssueConcept ;
              dcterms:issued "2024-09-30"^^xsd:date ;
              rdfs:comment """Added to the original framework. Inverse of ContextualizedCriterion in the original framework. Describes an instance of the bdqffdq:IssueConcept in terms of the associated bdqffdq:InformationElements from a controlled vocabulary (fields bdqffdq:ActedUpon or bdqffdq:Consulted), and a bdqffdq:ResourceType of bdqffdq:SingleRecord or bdqffdq:MultiRecord. Describes bdqffdq:Criteria by which data that lack quality for some purpose may be identified. A bdqffdq:Issue is phrased in a negative sense, and approximates an inverse of a bdqffdq:Validation. A bdqffdq:Issue identifies data that lack or may lack quality. A bdqffdq:Issue may flag a bdqffdq:POTENTIAL_ISSUE that would need further review to determine if the data have quality for some purpose. If the conditions described by a bdqffdq:Issue are identified by a Test, the bdqffdq:ResponseResult will be either bdqffdq:IS_ISSUE or bdqffdq:POTENTIAL_ISSUE, if no bdqffdq:Issue is found with the data, the bdqffdq:ResponseResult will be bdqffdq:NOT_ISSUE. The term bdqffdq:NOT_ISSUE, unlike bdqffdq:COMPLIANT for a bdqffdq:Validation, does not assert that data are fit for some purpose. A bdqffdq:Issue is the bdqffdq:DataQualityNeed concept that parallels a bdqffdq:IssueMethod in the Solutions layer (see Figure 3 in Veiga et al., 2017), and a bdqffdq:IssueAssertion in the Report layer (see Figure 3 in Veiga et al., 2017).

IS = { is | is = < ie, c, rt >, ie ∈ IE, c ∈ ∁C ⋀ rt ∈ RT }"""@en ;
              rdfs:label "Issue"@en ;
              skos:definition "A bdqffdq:DataQualityNeed that expresses how quality problems may be identified in data."@en ;
              skos:prefLabel "Issue"@en .


###  https://rs.tdwg.org/bdqffdq/terms/IssueAssertion
bdqffdq:IssueAssertion rdf:type owl:Class ;
                       rdfs:subClassOf bdqffdq:Assertion ,
                                       bdqffdq:IssueConcept ;
                       dcterms:issued "2024-09-30"^^xsd:date ;
                       rdfs:comment """The bdqffdq:DataQualityReport concept describing the result of a Test in the negative (i.e., identifying the potential absence of data quality). 

If a problem was found, the bdqffdq:ResponseResult is expected to carry a value of bdqffdq:IS_ISSUE, if a potential problem was found that requires human review, the bdqffdq:ResponseResult is expected to be bdqffdq:POTENTIAL_ISSUE, otherwise if the bdqffdq:ResponseStatus is bdqffdq:RUN_HAS_RESULT, the bdqffdq:ResponseResult is expected to be bdqffdq:NOT_ISSUE."""@en ;
                       rdfs:label "Issue Assertion"@en ;
                       skos:definition "A bdqffdq:Assertion expressing the result of a bdqffdq:Implementation evaluating a bdqffdq:Issue for a particular bdqffdq:DataQualityNeed in a particular bdqffdq:DataResource."@en ;
                       skos:prefLabel "Issue Assertion"@en .


###  https://rs.tdwg.org/bdqffdq/terms/IssueConcept
bdqffdq:IssueConcept rdf:type owl:Class ;
                     dcterms:issued "2024-09-30"^^xsd:date ;
                     rdfs:comment "A bdqffdq:Issue term is expressed in a negative sense, it identifies data that do not or may not conform to bdqffdq:DataQualityNeeds."@en ;
                     rdfs:label "Issue Concept"@en ;
                     skos:definition "A term involved in flagging problems or potential problems in assessment of data quality that would or might prevent the data from meeting an expressed bdqffdq:DataQualityNeed."@en ;
                     skos:prefLabel "Issue Concept"@en .


###  https://rs.tdwg.org/bdqffdq/terms/IssueMethod
bdqffdq:IssueMethod rdf:type owl:Class ;
                    rdfs:subClassOf bdqffdq:DataQualityMethod ,
                                    bdqffdq:IssueConcept ;
                    dcterms:issued "2024-09-30"^^xsd:date ;
                    rdfs:comment "A bdqffdq:IssueMethod is a data quality Solutions layer concept (see Figure 3 in Veiga et al., 2017) describing the relationship between a bdqffdq:Specification (technical description of a Test) and a bdqffdq:Issue (a bdqffdq:Criterion in the context of bdqffdq:ResourceType (bdqffdq:SingleRecord or bdqffdq:MultiRecord) and associated bdqffdq:InformationElements)."@en ;
                    rdfs:label "Issue Method"@en ;
                    skos:definition "A data quality bdqffdq:SolutionsConcept that relates a bdqffdq:Issue to its bdqffdq:Specifications."@en ;
                    skos:prefLabel "Issue Method"@en .


###  https://rs.tdwg.org/bdqffdq/terms/IssuePolicy
bdqffdq:IssuePolicy rdf:type owl:Class ;
                    rdfs:subClassOf bdqffdq:IssueConcept ,
                                    bdqffdq:Policy ;
                    dcterms:issued "2024-09-30"^^xsd:date ;
                    rdfs:comment "A bdqffdq:IssuePolicy is a data quality Need layer concept (see Figure 3 in Veiga et al., 2017) that describes how a bdqffdq:Issue relates to a bdqffdq:UseCase. This relationship defines which bdqffdq:Issues are supported by a given bdqffdq:UseCase."@en ;
                    rdfs:label "Issue Policy"@en ;
                    skos:definition "A bdqffdq:NeedConcept that relates a bdqffdq:UseCase to a set of supporting bdqffdq:Issues."@en ;
                    skos:prefLabel "Issue Policy"@en .


###  https://rs.tdwg.org/bdqffdq/terms/Measure
bdqffdq:Measure rdf:type owl:Class ;
                rdfs:subClassOf bdqffdq:DataQualityNeed ,
                                bdqffdq:MeasurementConcept ;
                dcterms:issued "2024-09-30"^^xsd:date ;
                rdfs:comment """ContextualizedDimension in the original framework. Describes an instance of the bdqffdq:MeasurementConcept in terms of the associated bdqffdq:InformationElements from a controlled vocabulary (fields bdqffdq:ActedUpon or bdqffdq:Consulted), and a bdqffdq:ResourceType of bdqffdq:SingleRecord or bdqffdq:MultiRecord. 

Describes the bdqffdq:Criteria for measuring an aspect of data quality related to a bdqffdq:DataQualityNeed. May be bdqffdq:Criteria for determining that data are bdqffdq:COMPLETE or bdqffdq:NOT_COMPLETE, or may be bdqffdq:Criteria for asserting a numeric bdqffdq:Measure. The bdqffdq:COMPLETE and bdqffdq:NOT_COMPLETE bdqffdq:Measures are fundamental to data quality control, as a set of data is filtered to the subset of data that have quality for some need if all records are bdqffdq:COMPLETE for all pertinent bdqffdq:Measures.

A bdqffdq:Measure is the bdqffdq:DataQualityNeed concept that parallels a bdqffdq:MeasurementMethod in the Solutions layer (see Figure 3 in Veiga et al., 2017), and a bdqffdq:MeasurementAssertion in the Report layer (see Figure 3 in Veiga et al., 2017).

ME = { me | me =< ie, d, rt >, ie ∈ IE, d ∈ D ⋀ rt ∈ RT }
also acceptable bdqffdq:Measure
AM(me) = {va | me ∈ C D ⋀ va ⊂ C C}"""@en ;
                rdfs:label "Measure"@en ;
                skos:definition "A bdqffdq:DataQualityNeed that expresses how the fitness of data for some use may be measured."@en ;
                skos:prefLabel "Measure"@en .


###  https://rs.tdwg.org/bdqffdq/terms/MeasurementAssertion
bdqffdq:MeasurementAssertion rdf:type owl:Class ;
                             rdfs:subClassOf bdqffdq:Assertion ,
                                             bdqffdq:MeasurementConcept ;
                             dcterms:issued "2024-09-30"^^xsd:date ;
                             rdfs:comment """A bdqffdq:MeasurementAssertion is a Report layer concept (see Figure 3 in Veiga et al., 2017) that describes the results of the execution of a Test that performs a bdqffdq:MeasurementMethod following a bdqffdq:Specification to assess a data quality bdqffdq:Measure. 

A MeasurementAssertion is expected to carry a bdqffdq:ResponseResult of bdqffdq:COMPLETE or bdqffdq:NOT_COMPLETE or a numeric measured value (e.g., a bdqffdq:Measure of a dwc:eventDate duration in seconds).

DQM(dr) = {dqm | dqm =< me, s, m, r >, me ∈ ME, s ∈ S, m ∈ M , r ∈ R ⋀ dr ∈ DR}"""@en ;
                             rdfs:label "Measurement Assertion"@en ;
                             skos:definition "A bdqffdq:Assertion expressing the result of a bdqffdq:Implementation measuring a particular bdqffdq:DataQualityNeed in a particular bdqffdq:DataResource."@en ;
                             skos:prefLabel "Measurement Assertion"@en .


###  https://rs.tdwg.org/bdqffdq/terms/MeasurementConcept
bdqffdq:MeasurementConcept rdf:type owl:Class ;
                           dcterms:issued "2024-09-30"^^xsd:date ;
                           rdfs:label "Measurement Concept"@en ;
                           skos:definition "A term involved in measurement of data quality with regards to expressed bdqffdq:DataQualityNeed."@en ;
                           skos:prefLabel "Measurement Concept"@en .


###  https://rs.tdwg.org/bdqffdq/terms/MeasurementMethod
bdqffdq:MeasurementMethod rdf:type owl:Class ;
                          rdfs:subClassOf bdqffdq:DataQualityMethod ,
                                          bdqffdq:MeasurementConcept ;
                          dcterms:issued "2024-09-30"^^xsd:date ;
                          rdfs:comment """A bdqffdq:MeasurementMethod is a data quality Solutions layer concept (see Figure 3 in Veiga et al., 2017) describing the relationship between a bdqffdq:Specification (technical description of a Test) and a bdqffdq:Measurement (a bdqffdq:Dimension in the context of bdqffdq:ResourceType (bdqffdq:SingleRecord or bdqffdq:MultiRecord) and associated bdqffdq:InformationElements).

MM(me) = {s | s ⊂ S ⋀ me ∈ ME}"""@en ;
                          rdfs:label "Measurement Method"@en ;
                          skos:definition "A data quality bdqffdq:SolutionsConcept that relates a bdqffdq:Measure to its bdqffdq:Specifications."@en ;
                          skos:prefLabel "Measurement Method"@en .


###  https://rs.tdwg.org/bdqffdq/terms/MeasurementPolicy
bdqffdq:MeasurementPolicy rdf:type owl:Class ;
                          rdfs:subClassOf bdqffdq:MeasurementConcept ,
                                          bdqffdq:Policy ;
                          dcterms:issued "2024-09-30"^^xsd:date ;
                          rdfs:comment """A bdqffdq:MeasurementPolicy is a data quality Need layer concept (see Figure 3 in Veiga et al., 2017) that describes how a bdqffdq:Measurement relates to a bdqffdq:UseCase. This relationship defines which bdqffdq:Measures are supported by a given bdqffdq:UseCase.

MP(u) = {me | me ⊂ ME ⋀ u ∈ U }"""@en ;
                          rdfs:label "Measurement Policy"@en ;
                          skos:definition "A bdqffdq:NeedConcept that relates a bdqffdq:UseCase to a set of supporting bdqffdq:Measures."@en ;
                          skos:prefLabel "Measurement Policy"@en .


###  https://rs.tdwg.org/bdqffdq/terms/Mechanism
bdqffdq:Mechanism rdf:type owl:Class ;
                  rdfs:subClassOf bdqffdq:FundamentalConcept ,
                                  bdqffdq:SolutionsConcept ;
                  dcterms:issued "2024-09-30"^^xsd:date ;
                  rdfs:comment """A bdqffdq:Mechanism may produce bdqffdq:DataQualityReports as products.

A bdqffdq:Mechanism describes the entity that performs a bdqffdq:Assertion Test (code, external service, actor, etc.). Tied to a bdqffdq:Specification via the concept of a bdqffdq:Implementation."""@en ;
                  rdfs:label "Mechanism"@en ;
                  skos:definition "An entity that can execute bdqffdq:DataQualityMethods."@en ;
                  skos:prefLabel "Mechanism"@en .


###  https://rs.tdwg.org/bdqffdq/terms/NeedConcept
bdqffdq:NeedConcept rdf:type owl:Class ;
                    dcterms:issued "2024-09-30"^^xsd:date ;
                    rdfs:comment "Category of concepts forming the Need layer of the fitness for use framework (see Figure 3 in Veiga et al., 2017)."@en ;
                    rdfs:label "Need Concept"@en ;
                    skos:definition "A concept that expresses an aspect of a bdqffdq:DataQualityNeed."@en ;
                    skos:prefLabel "Need Concept"@en .


###  https://rs.tdwg.org/bdqffdq/terms/Parameter
bdqffdq:Parameter rdf:type owl:Class ;
                  rdfs:subClassOf bdqffdq:SolutionsConcept ;
                  dcterms:issued "2024-09-30"^^xsd:date ;
                  rdfs:comment "A bdqffdq:Parameter is a Formal Parameter for which an bdqffdq:Argument is an Actual Parameter that replaces it to determine the behavior of a bdqffdq:Specification. An extension to the original fitness for use framework as described in Veiga et al., 2017."@en ;
                  rdfs:label "Parameter"@en ;
                  skos:definition "A placeholder for a value that, when provided to a Test bdqffdq:Specification changes the behavior of the Test in a defined manner."@en ;
                  skos:prefLabel "Parameter"@en .


###  https://rs.tdwg.org/bdqffdq/terms/Policy
bdqffdq:Policy rdf:type owl:Class ;
               rdfs:subClassOf bdqffdq:NeedConcept ;
               dcterms:issued "2024-09-30"^^xsd:date ;
               rdfs:comment "Composition of bdqffdq:DataQualityNeeds into a bdqffdq:UseCase."@en ;
               rdfs:label "Policy"@en ;
               skos:definition "The set of bdqffdq:DataQualityNeeds for a bdqffdq:UseCase."@en ;
               skos:prefLabel "Policy"@en .


###  https://rs.tdwg.org/bdqffdq/terms/ReportConcept
bdqffdq:ReportConcept rdf:type owl:Class ;
                      dcterms:issued "2024-09-30"^^xsd:date ;
                      rdfs:comment "Category of concepts forming the Report layer of the fitness for use framework (see Figure 3 in Veiga et al., 2017)."@en ;
                      rdfs:label "Report Concept"@en ;
                      skos:definition "A concept concerning data quality expressed in a bdqffdq:DataQualityReport."@en ;
                      skos:prefLabel "Report Concept"@en .


###  https://rs.tdwg.org/bdqffdq/terms/ResourceType
bdqffdq:ResourceType rdf:type owl:Class ;
                     rdfs:subClassOf bdqffdq:FundamentalConcept ;
                     dcterms:issued "2024-09-30"^^xsd:date ;
                     rdfs:comment "The concept of bdqffdq:ResourceType has instances for bdqffdq:SingleRecord or bdqffdq:MultiRecord."@en ;
                     rdfs:label "Resource Type"@en ;
                     skos:definition "Category of things that are data objects about which data quality bdqffdq:Assertions may be made."@en ;
                     skos:prefLabel "Resource Type"@en .


###  https://rs.tdwg.org/bdqffdq/terms/ResponseQualifier
bdqffdq:ResponseQualifier rdf:type owl:Class ;
                          rdfs:subClassOf bdqffdq:ReportConcept ;
                          dcterms:issued "2024-09-30"^^xsd:date ;
                          rdfs:comment "Intended as an extension point for qualifying information about uncertainty or ambiguity."@en ;
                          rdfs:label "Response Qualifier"@en ;
                          skos:definition "A bdqffdq:ReportConcept to which additional bdqffdq:Assertions providing additional information beyond that of bdqffdq:ResponseResult from the execution of the bdqffdq:Specification of a bdqffdq:DataQualityNeed are attached."@en ;
                          skos:prefLabel "Response Qualifier"@en .


###  https://rs.tdwg.org/bdqffdq/terms/ResponseResult
bdqffdq:ResponseResult rdf:type owl:Class ;
                       rdfs:subClassOf bdqffdq:ReportConcept ;
                       dcterms:issued "2024-09-30"^^xsd:date ;
                       rdfs:comment """For a bdqffdq:Validation, a bdqffdq:ResponseResult may be bdqffdq:COMPLIANT, or bdqffdq:NOT_COMPLIANT. For a bdqffdq:Measure, a bdqffdq:ResponseResult object may be bdqffdq:COMPLETE or bdqffdq:NOT_COMPLETE. For a bdqffdq:Issue, a bdqffdq:ResponseResult may be bdqffdq:IS_ISSUE, bdqffdq:POTENTIAL_ISSUE, or bdqffdq:NOT_ISSUE. A bdqffdq:Measure may also use a numeric data property. A bdqffdq:Amendment asserts a string data property.

The bdqffdq:ResponseResult is represented as a value or a result object for bdqffdq:MeasureAsssertions, or just a result object for bdqffdq:ValidationAssertions or just values for changes proposed in bdqffdq:AmendmentAssertions."""@en ;
                       rdfs:label "Response.result"@en ;
                       skos:definition "A bdqffdq:ReportConcept to which controlled vocabulary bdqffdq:Assertions about the result of the execution of the bdqffdq:Specification of a bdqffdq:DataQualityNeed are attached."@en ;
                       skos:prefLabel "Response.result"@en .


###  https://rs.tdwg.org/bdqffdq/terms/ResponseStatus
bdqffdq:ResponseStatus rdf:type owl:Class ;
                       rdfs:subClassOf bdqffdq:ReportConcept ;
                       dcterms:issued "2024-09-30"^^xsd:date ;
                       rdfs:comment "The bdqffdq:ResponseStatus is metadata, indicating if data should be present in a bdqffdq:ResponseResult. Any bdqffdq:Assertion may have the values bdqffdq:INTERNAL_PREREQUISITES_NOT_MET or bdqffdq:EXTERNAL_PREREQUISITES_NOT_MET, indicating that no value would be present in the accompanying bdqffdq:ResponseResult. Other values depend on the bdqffdq:Assertion type; bdqffdq:RUN_HAS_RESULT for a bdqffdq:Validation, bdqffdq:Issue or bdqffdq:Measure, and bdqffdq:FILLED_IN, bdqffdq:AMENDED, or bdqffdq:NOT_AMENDED for a bdqffdq:Amendment. Additional metadata qualifying the bdqffdq:Assertion in a bdqffdq:ResponseResult, such as statements of uncertainy or ambiguity may be placed in the bdqffdq:ResponseQualifier."@en ;
                       rdfs:label "Response.status"@en ;
                       skos:definition "A bdqffdq:ReportConcept expressing controlled vocabulary values about the exit state of an execution process of a data quality bdqffdq:Specification by a bdqffdq:Implementation."@en ;
                       skos:prefLabel "Response.status"@en .


###  https://rs.tdwg.org/bdqffdq/terms/SolutionsConcept
bdqffdq:SolutionsConcept rdf:type owl:Class ;
                         dcterms:issued "2024-09-30"^^xsd:date ;
                         rdfs:comment "Category of concepts forming the Solutions layer of the fitness for use framework (see Figure 3 in Veiga et al., 2017). A bdqffdq:SolutionsConcept is a tool that evaluates data against bdqffdq:NeedConcepts and express conclusions in bdqffdq:DataQualityReports."@en ;
                         rdfs:label "Solutions Concept"@en ;
                         skos:definition "A concept that expresses an aspect of a data quality solution."@en ;
                         skos:prefLabel "Solutions Concept"@en .


###  https://rs.tdwg.org/bdqffdq/terms/Specification
bdqffdq:Specification rdf:type owl:Class ;
                      rdfs:subClassOf bdqffdq:FundamentalConcept ,
                                      bdqffdq:SolutionsConcept ;
                      dcterms:issued "2024-09-30"^^xsd:date ;
                      rdfs:comment "A bdqffdq:Specification is a technical description of a bdqffdq:Assertion Test. A bdqffdq:Specification is expected to have the following properties:  (1) bdqffdq:hasExpectedResponse and (2) bdqffdq:hasAuthoritiesDefaults."@en ;
                      rdfs:label "Specification"@en ;
                      skos:definition "A specific statement about how to evaluate a bdqffdq:DataQualityNeed."@en ;
                      skos:prefLabel "Specification"@en .


###  https://rs.tdwg.org/bdqffdq/terms/UseCase
bdqffdq:UseCase rdf:type owl:Class ;
                rdfs:subClassOf bdqffdq:FundamentalConcept ,
                                bdqffdq:NeedConcept ;
                dcterms:issued "2024-09-30"^^xsd:date ;
                rdfs:comment "A bdqffdq:UseCase describes a data quality control use case. The bdqffdq:ValidationPolicies, bdqffdq:MeasurementPolicies and bdqffdq:AmendmentPolicies that make up a bdqffdq:UseCase define which bdqffdq:Assertions cover a given bdqffdq:UseCase. An example of a bdqffdq:UseCase could be 'Check for internal consistency of dates', with bdqffdq:ValidationPolicies for checking consistency between atomic date fields and a bdqffdq:Amendment such as 'eventDate filled in from verbatim'. A bdqffdq:UseCase is not the same as a use cases in the software engineering sense, it is a similar formal bdqffdq: statement derived from analyis of user stories."@en ;
                rdfs:label "Use Case"@en ;
                skos:definition "A bdqffdq:NeedConcept expressing a purpose to which data are put for which the data must have quality for the result to have meaning and reliability."@en ;
                skos:prefLabel "Use Case"@en .


###  https://rs.tdwg.org/bdqffdq/terms/Validation
bdqffdq:Validation rdf:type owl:Class ;
                   rdfs:subClassOf bdqffdq:DataQualityNeed ,
                                   bdqffdq:ValidationConcept ;
                   dcterms:issued "2024-09-30"^^xsd:date ;
                   rdfs:comment """ContextualizedCriterion in the original framework. Describes the bdqffdq:Criteria for determining compliance of data to fill a bdqffdq:DataQualityNeed. A description of a bdqffdq:Criterion applied to a bdqffdq:InformationElement for a bdqffdq:ResourceType. Describes an instance of a bdqffdq:Criterion in terms of the associated bdqffdq:InformationElements from a controlled vocabulary (fields bdqffdq:ActedUpon or bdqffdq:Consulted), and a bdqffdq:ResourceType of bdqffdq:SingleRecord or bdqffdq:MultiRecord.

A bdqffdq:Validation is phrased in a positive sense. It identifies data which have quality for some need. For example, the value of dwc:basisOfRecord of bdqffdq:SingleRecords must be in the controlled vocabulary for dwc:basisOfRecord.

A bdqffdq:Validation is the bdqffdq:DataQualityNeed that parallels a bdqffdq:ValidationMethod in the Solutions layer (see Figure 3 in Veiga et al., 2017), and a bdqffdq:ValidationAssertion in the Report layer (see Figure 3 in Veiga et al., 2017). A bdqffdq:ValidationAssertion may specify a result that is bdqffdq:COMPLIANT, where the data have quality, or bdqffdq:NOT_COMPLIANT, where the data lack quality for a bdqffdq:UseCase.

VA = { va | va = < ie, c, rt >, ie ∈ IE, c ∈ C ⋀ rt ∈ RT }"""@en ;
                   rdfs:label "Validation"@en ;
                   skos:definition "A bdqffdq:DataQualityNeed that expresses how data may be evaluated for fitness for use."@en ;
                   skos:prefLabel "Validation"@en .


###  https://rs.tdwg.org/bdqffdq/terms/ValidationAssertion
bdqffdq:ValidationAssertion rdf:type owl:Class ;
                            rdfs:subClassOf bdqffdq:Assertion ,
                                            bdqffdq:ValidationConcept ;
                            dcterms:issued "2024-09-30"^^xsd:date ;
                            rdfs:comment """The bdqffdq:ValidationAssertion is a Report layer concept (see Figure 3 in Veiga et al., 2017) that describes the results of the execution of a Test that performs a bdqffdq:ValidationMethod following a bdqffdq:Specification to assess the validity of some data with respect to the bdqffdq:Criteria of a bdqffdq:Validation. 

The bdqffdq:ValidationAssertion concept is expected to carry a bdqffdq:ResponseResult of bdqffdq:COMPLIANT or bdqffdq:NON_COMPLIANT.

DQV(dr) = {dqv | dqv = < va, s, m, r >, va ∈ VA, s ∈ S, m ∈ M , r ∈ R ⋀ dr ∈ DR}"""@en ;
                            rdfs:label "Validation Assertion"@en ;
                            skos:definition "A bdqffdq:Assertion expressing the result of a bdqffdq:Implementation validating compliance with a particular bdqffdq:DataQualityNeed in a particular bdqffdq:DataResource."@en ;
                            skos:prefLabel "Validation Assertion"@en .


###  https://rs.tdwg.org/bdqffdq/terms/ValidationConcept
bdqffdq:ValidationConcept rdf:type owl:Class ;
                          dcterms:issued "2024-09-30"^^xsd:date ;
                          rdfs:comment "A bdqffdq:Validation term is expressed in a positive sense, it identifies data that conform to a bdqffdq:NeedConcept."@en ;
                          rdfs:label "Validation Concept"@en ;
                          skos:definition "A term involved in statements about the conformance of data to expressed bdqffdq:DataQualityNeeds."@en ;
                          skos:prefLabel "Validation Concept"@en .


###  https://rs.tdwg.org/bdqffdq/terms/ValidationMethod
bdqffdq:ValidationMethod rdf:type owl:Class ;
                         rdfs:subClassOf bdqffdq:DataQualityMethod ,
                                         bdqffdq:ValidationConcept ;
                         dcterms:issued "2024-09-30"^^xsd:date ;
                         rdfs:comment """A bdqffdq:ValidationMethod is a data quality Solutions layer concept (see Figure 3 in Veiga et al., 2017) describing the relationship between a bdqffdq:Specification (technical description of a Test) and a bdqffdq:Validation (a bdqffdq:Criterion in the context of bdqffdq:ResourceType (bdqffdq:SingleRecord or bdqffdq:MultiRecord) and associated bdqffdq:InformationElements).

VM(va) = {s | s ⊂ S ⋀ va ∈ VA}"""@en ;
                         rdfs:label "Validation Method"@en ;
                         skos:definition "A data quality bdqffdq:SolutionsConcept that relates a bdqffdq:Validation to its bdqffdq:Specifications."@en ;
                         skos:prefLabel "Validation Method"@en .


###  https://rs.tdwg.org/bdqffdq/terms/ValidationPolicy
bdqffdq:ValidationPolicy rdf:type owl:Class ;
                         rdfs:subClassOf bdqffdq:Policy ,
                                         bdqffdq:ValidationConcept ;
                         dcterms:issued "2024-09-30"^^xsd:date ;
                         rdfs:comment """A bdqffdq:ValidationPolicy is a data quality Need layer concept (see Figure 3 in Veiga et al., 2017) that describes how a bdqffdq:Validation relates to a bdqffdq:UseCase. This relationship defines which bdqffdq:Validations are needed to identify quality in a given bdqffdq:UseCase.

VP (u) = {va | va ⊂ VA ⋀ u ∈ U }"""@en ;
                         rdfs:label "Validation Policy"@en ;
                         skos:definition "A bdqffdq:NeedConcept that relates a bdqffdq:UseCase to a set of supporting bdqffdq:Validations."@en ;
                         skos:prefLabel "Validation Policy"@en .


#################################################################
#    Individuals
#################################################################

###  https://rs.tdwg.org/bdqffdq/terms/AMENDED
bdqffdq:AMENDED rdf:type owl:NamedIndividual ,
                         bdqffdq:ResponseStatus ;
                owl:differentFrom bdqffdq:NOT_AMENDED ;
                dcterms:issued "2024-09-30"^^xsd:date ;
                rdf:value "AMENDED" ;
                rdfs:comment "The value bdqffdq:AMENDED implies that a change is being proposed to an existing bdq:NotEmpty value. bdqffdq:Amendments do not provide bdqffdq:hasResponseResult object properties. Proposed changes will be in a bdqffdq:hasResponseResultValue data property."@en ;
                rdfs:label "AMENDED"@en ;
                skos:definition "A bdqffdq:ResponseStatus used to indicate that a bdqffdq:hasResponseResultValue from a bdqffdq:Amendment contains a proposed change."@en ;
                skos:prefLabel "AMENDED"@en .


###  https://rs.tdwg.org/bdqffdq/terms/COMPLETE
bdqffdq:COMPLETE rdf:type owl:NamedIndividual ,
                          bdqffdq:ResponseResult ;
                 owl:differentFrom bdqffdq:NOT_COMPLETE ;
                 dcterms:issued "2024-09-30"^^xsd:date ;
                 rdf:value "COMPLETE" ;
                 rdfs:comment "This value can be used to filter data for Quality Assurance. This value can be asserted, for example, by bdqffdq:Measures of bdqffdq:MultiRecords where all the bdqffdq:Validation bdqffdq:ResponseResults from all included records in the dataset are bdqffdq:COMPLIANT."@en ;
                 rdfs:label "COMPLETE"@en ;
                 skos:definition "A bdqffdq:ResponseResult of a bdqffdq:Measure that asserts that data are present and sufficiently comprehensive for use." ;
                 skos:prefLabel "COMPLETE"@en .


###  https://rs.tdwg.org/bdqffdq/terms/COMPLIANT
bdqffdq:COMPLIANT rdf:type owl:NamedIndividual ,
                           bdqffdq:ResponseResult ;
                  owl:differentFrom bdqffdq:NOT_COMPLIANT ;
                  dcterms:issued "2024-09-30"^^xsd:date ;
                  rdf:value "COMPLIANT" ;
                  rdfs:label "COMPLIANT"@en ;
                  skos:definition "A bdqffdq:ResponseResult of a bdqffdq:Validation where the data conforms to the bdqffdq:Criteria for quality in the Test bdqffdq:Specification."@en ;
                  skos:prefLabel "COMPLIANT"@en .


###  https://rs.tdwg.org/bdqffdq/terms/EXTERNAL_PREREQUISITES_NOT_MET
bdqffdq:EXTERNAL_PREREQUISITES_NOT_MET rdf:type owl:NamedIndividual ,
                                                bdqffdq:ResponseStatus ;
                                       owl:differentFrom bdqffdq:INTERNAL_PREREQUISITES_NOT_MET ;
                                       dcterms:issued "2024-09-30"^^xsd:date ;
                                       rdf:value "EXTERNAL_PREREQUISITES_NOT_MET" ;
                                       rdfs:label "EXTERNAL_PREREQUISITES_NOT_MET"@en ;
                                       skos:definition "A bdqffdq:ResponseStatus used to indicate that a bdqffdq:ResponseResult was not generated because a bdq:sourceAuthority was not accessible. If the Test is run at a later time, it may produce a different bdqffdq:ResponseStatus."@en ;
                                       skos:prefLabel "EXTERNAL_PREREQUISITES_NOT_MET"@en .


###  https://rs.tdwg.org/bdqffdq/terms/FILLED_IN
bdqffdq:FILLED_IN rdf:type owl:NamedIndividual ,
                           bdqffdq:ResponseStatus ;
                  owl:differentFrom bdqffdq:NOT_AMENDED ;
                  dcterms:issued "2024-09-30"^^xsd:date ;
                  rdf:value "FILLED_IN" ;
                  rdfs:label "FILLED_IN"@en ;
                  skos:definition "A bdqffdq:ResponseStatus used to indicate that a bdqffdq:Amendment contains a proposed change to a record in a bdqffdq:hasResponseResultValue where the bdqffdq:InformationElement was bdq:Empty."@en ;
                  skos:prefLabel "FILLED_IN"@en .


###  https://rs.tdwg.org/bdqffdq/terms/INTERNAL_PREREQUISITES_NOT_MET
bdqffdq:INTERNAL_PREREQUISITES_NOT_MET rdf:type owl:NamedIndividual ,
                                                bdqffdq:ResponseStatus ;
                                       dcterms:issued "2024-09-30"^^xsd:date ;
                                       rdf:value "INTERNAL_PREREQUISITES_NOT_MET" ;
                                       rdfs:label "INTERNAL_PREREQUISITES_NOT_MET"@en ;
                                       skos:definition "A bdqffdq:ResponseStatus used to indicate that a bdqffdq:ResponseResult was not generated because values of the bdqffdq:InformationElement were insufficient to run the Test. If the Test is run at a later time on unmodified data, it should produce the same bdqffdq:ResponseStatus."@en ;
                                       skos:prefLabel "INTERNAL_PREREQUISITES_NOT_MET"@en .


###  https://rs.tdwg.org/bdqffdq/terms/IS_ISSUE
bdqffdq:IS_ISSUE rdf:type owl:NamedIndividual ,
                          bdqffdq:ResponseResult ;
                 owl:differentFrom bdqffdq:NOT_ISSUE ,
                                   bdqffdq:POTENTIAL_ISSUE ;
                 dcterms:issued "2024-09-30"^^xsd:date ;
                 rdf:value "IS_ISSUE" ;
                 rdfs:comment "This is a parallel bdqffdq:ResponseResult to bdqffdq:NOT_COMPLIANT"@en ;
                 rdfs:label "IS_ISSUE"@en ;
                 skos:definition "A bdqffdq:ResponseResult of a bdqffdq:Issue indicating that the data do not have sufficient quality for a use."@en ;
                 skos:prefLabel "IS_ISSUE"@en .


###  https://rs.tdwg.org/bdqffdq/terms/MultiRecord
bdqffdq:MultiRecord rdf:type owl:NamedIndividual ,
                             bdqffdq:ResourceType ;
                    dcterms:issued "2024-09-30"^^xsd:date ;
                    rdfs:comment "A data set. Encoded data with a defined structure that can be described as dcmitype:Dataset."@en ;
                    rdfs:label "Multi Record"@en ;
                    skos:definition "A set of one or more bdqffdq:SingleRecords."@en ;
                    skos:prefLabel "Multi Record"@en .


###  https://rs.tdwg.org/bdqffdq/terms/NOT_AMENDED
bdqffdq:NOT_AMENDED rdf:type owl:NamedIndividual ,
                             bdqffdq:ResponseStatus ;
                    dcterms:issued "2024-09-30"^^xsd:date ;
                    rdf:value "NOT_AMENDED" ;
                    rdfs:comment "No value will be provided in a bdqfdq:hasResponseResultValue. bdqffdq:Amendments do not provide bdqffdq:hasResponseResult object properties."@en ;
                    rdfs:label "NOT_AMENDED"@en ;
                    skos:definition "A bdqffdq:ResponseStatus used to indicate that a bdqffdq:Amendment proposed no change."@en ;
                    skos:prefLabel "NOT_AMENDED"@en .


###  https://rs.tdwg.org/bdqffdq/terms/NOT_COMPLETE
bdqffdq:NOT_COMPLETE rdf:type owl:NamedIndividual ,
                              bdqffdq:ResponseResult ;
                     dcterms:issued "2024-09-30"^^xsd:date ;
                     rdf:value "NOT_COMPLETE" ;
                     rdfs:comment "This value can be used to exclude data for Quality Assurance. This value can be asserted, for example, by bdqffdq:Measures of bdqffdq:MultiRecords where not all the bdqffdq:Validation bdqffdq:ResponseResult from all included records in the dataset have a bdqffdq:ResponseResult of bdqffdq:COMPLIANT."@en ;
                     rdfs:label "NOT_COMPLETE"@en ;
                     skos:definition "A bdqffdq:ResponseResult of a bdqffdq:Measure which asserts that data are not present or are not sufficiently comprehensive for a use."@en ;
                     skos:prefLabel "NOT_COMPLETE"@en .


###  https://rs.tdwg.org/bdqffdq/terms/NOT_COMPLIANT
bdqffdq:NOT_COMPLIANT rdf:type owl:NamedIndividual ,
                               bdqffdq:ResponseResult ;
                      dcterms:issued "2024-09-30"^^xsd:date ;
                      rdf:value "NOT_COMPLIANT" ;
                      rdfs:label "NOT_COMPLIANT"@en ;
                      skos:definition "A bdqffdq:ResponseResult of a bdqffdq:Validation where the data do not conform to the bdqffdq:Criteria for quality in the Test bdqffdq:Specification."@en ;
                      skos:prefLabel "NOT_COMPLIANT"@en .


###  https://rs.tdwg.org/bdqffdq/terms/NOT_ISSUE
bdqffdq:NOT_ISSUE rdf:type owl:NamedIndividual ,
                           bdqffdq:ResponseResult ;
                  owl:differentFrom bdqffdq:POTENTIAL_ISSUE ;
                  dcterms:issued "2024-09-30"^^xsd:date ;
                  rdf:value "NOT_ISSUE" ;
                  rdfs:comment "This is similar to, but has different semantics to, bdqffdq:COMPLIANT for a bdqffdq:Validation. The value bdqffdq:COMPLIANT means that the data were evaluated as having quality according to a bdqffdq:Criterion. The value bdqffdq:NOT_ISSUE means that no bdqffdq:Issue with data quality was found under a bdqffdq:Criterion for identifying the absence of quality."@en ;
                  rdfs:label "NOT_ISSUE"@en ;
                  skos:definition "A bdqffdq:ResponseResult of a bdqffdq:Issue where no potential problems were detected."@en ;
                  skos:prefLabel "NOT_ISSUE"@en .


###  https://rs.tdwg.org/bdqffdq/terms/POTENTIAL_ISSUE
bdqffdq:POTENTIAL_ISSUE rdf:type owl:NamedIndividual ,
                                 bdqffdq:ResponseResult ;
                        dcterms:issued "2024-09-30"^^xsd:date ;
                        rdf:value "POTENTIAL_ISSUE" ;
                        rdfs:comment "See also bdqffdq:IS_ISSUE and bdqffdq:NOT_ISSUE. The value bdqffdq:POTENTIAL_ISSUE has no analog in a bdqffdq:Validation."@en ;
                        rdfs:label "POTENTIAL_ISSUE"@en ;
                        skos:definition "A bdqffdq:ResponseResult of a bdqffdq:Issue that indicates that the data may not have sufficient quality for a use. The user will need to evaluate if the data are fit for their particular use or not."@en ;
                        skos:prefLabel "POTENTIAL_ISSUE"@en .


###  https://rs.tdwg.org/bdqffdq/terms/RUN_HAS_RESULT
bdqffdq:RUN_HAS_RESULT rdf:type owl:NamedIndividual ,
                                bdqffdq:ResponseStatus ;
                       dcterms:issued "2024-09-30"^^xsd:date ;
                       rdf:value "RUN_HAS_RESULT" ;
                       rdfs:comment "Applies to bdqffdq:Validations, bdqffdq:Issues and bdqfdfq:Measures, but not bdqffdq:Amendments. For a bdqffdq:Validation or a bdqffdq:Issue, the value will be found as a bdqffdq:ResponseResult object by following bdqffdq:hasResponseResult. For a bdqffdq:Measure, the value could be either in the data property bdqffdq:hasResponseResultValue or could be a ResponseResult object."@en ;
                       rdfs:label "RUN_HAS_RESULT"@en ;
                       skos:definition "A bdqffdq:ResponseStatus used to indicate that that a result was correctly generated."@en ;
                       skos:prefLabel "RUN_HAS_RESULT"@en .


###  https://rs.tdwg.org/bdqffdq/terms/SingleRecord
bdqffdq:SingleRecord rdf:type owl:NamedIndividual ,
                              bdqffdq:ResourceType ;
                     dcterms:issued "2024-09-30"^^xsd:date ;
                     rdfs:comment """A record from a dcmitype:Dataset. May be a database tuple, in the strict sense (i.e, a single row in a table) or may be rows related across several tables, or a graph of data. A bdqffdq:SingleRecord is single in that it has one instance of a core concept from the perspective of bdqffdq:InformationElements assessed for a bdqffdq:UseCase. For example, in a bdqffdq:UseCase where dwc:Occurences are central, a bdqffdq:SingleRecord would represent a single dwc:Occurrence, but could have multiple dwc:Identifications and multiple dwc:Taxa related to it in a graph or data structure. However, in a bdqffdq:UseCase where dwc:Taxa are central, a bdqffdq:SingleRecord would represent a single dwc:Taxon entity (and might have multiple dwc:Occurrences related to it as part of the bdqffdq:SingleRecord, so long as the graph was limited before reaching other dwc:Taxon entities).

A bdqffdq:SingleRecord, like a bdqffdq:MultiRecord, consists of data with a defined structure that can be described as dcmitype:Dataset"""@en ;
                     rdfs:label "Single Record"@en ;
                     skos:definition "A single entity comprised of encoded data with a defined structure that contains one instance of a core concept from the perspective of bdqffdq:InformationElements assessed for a bdqffdq:DataQualityNeed."@en ;
                     skos:prefLabel "Single Record"@en .


#################################################################
#    General axioms
#################################################################

[ rdf:type owl:AllDisjointClasses ;
  owl:members ( bdqffdq:AbstractInformationElement
                bdqffdq:ActedUpon
                bdqffdq:Consulted
              )
] .


[ rdf:type owl:AllDisjointClasses ;
  owl:members ( bdqffdq:Amendment
                bdqffdq:Issue
                bdqffdq:Measure
                bdqffdq:Validation
              )
] .


###  Generated by the OWL API (version 4.5.29.2024-05-13T12:11:03Z) https://github.com/owlcs/owlapi
